theories/Unshadow.v
@@ -13,57 +13,60 @@ From LinearCore Require Import
 
 (* NOTE: Even though it's a very unusual case, this has to return an option
  * because patterns (in `Cas`) can be ill-formed if they duplicate a binder. *)
-Fixpoint unshadow_acc (acc : Map.to String.string) (reserved : Map.set) t :=
+Fixpoint unshadow_acc (acc : Map.to String.string) (cant_bind : Map.set) t :=
   match t with
-  | Term.Ctr ctor => Some (reserved, Term.Ctr ctor)
+  | Term.Ctr ctor => Some (cant_bind, Term.Ctr ctor)
   | Term.Var k ownership =>
       (* Have to supply a plan for any free variables (or they have to have been bound & added to the plan): *)
-      match Map.find acc k with None => None | Some v => Some (reserved, Term.Var v ownership) end
+      match Map.find acc k with None => None | Some v => Some (cant_bind, Term.Var v ownership) end
   | Term.App f a =>
-      match unshadow_acc acc reserved f with None => None | Some (reserved, f') =>
-        match unshadow_acc acc reserved a with None => None | Some (reserved, a') =>
-          Some (reserved, Term.App f' a')
+      match unshadow_acc acc cant_bind f with None => None | Some (cant_bind, f') =>
+        match unshadow_acc acc cant_bind a with None => None | Some (cant_bind, a') =>
+          Some (cant_bind, Term.App f' a')
         end
       end
   | Term.For variable type body =>
-      match unshadow_acc acc reserved type with None => None | Some (reserved, type') =>
-        let variable' := NewNames.new_name reserved variable in
+      match unshadow_acc acc cant_bind type with None => None | Some (cant_bind, type') =>
+        let variable' := NewNames.new_name cant_bind variable in
         let acc := Map.overwrite variable variable' acc in
-        let reserved := Map.set_add variable' reserved in
-        match unshadow_acc acc reserved body with None => None | Some (reserved, body') =>
-          Some (reserved, Term.For variable' type' body')
+        let cant_bind := Map.set_add variable' cant_bind in
+        match unshadow_acc acc cant_bind body with None => None | Some (cant_bind, body') =>
+          Some (cant_bind, Term.For variable' type' body')
         end
       end
   | Term.Cas pattern body_if_match other_cases =>
-      match unshadow_acc acc reserved other_cases with None => None | Some (reserved, other_cases') =>
+      match unshadow_acc acc cant_bind other_cases with None => None | Some (cant_bind, other_cases') =>
         let bindings := BoundIn.pattern pattern in
-        let rebindings := NewNames.generate reserved bindings in
+        let rebindings := NewNames.generate cant_bind bindings in
         match Rename.pattern rebindings pattern with
         | None => None
         | Some pattern' =>
             let acc := Map.bulk_overwrite rebindings acc in
-            let reserved := Map.set_union (Map.range rebindings) reserved in
-            match unshadow_acc acc reserved body_if_match with None => None | Some (reserved, body_if_match') =>
-              Some (reserved, Term.Cas pattern' body_if_match' other_cases')
+            let cant_bind := Map.set_union (Map.range rebindings) cant_bind in
+            match unshadow_acc acc cant_bind body_if_match with None => None | Some (cant_bind, body_if_match') =>
+              Some (cant_bind, Term.Cas pattern' body_if_match' other_cases')
             end
         end
       end
   end.
 
-Definition unshadow_reserve reserved t :=
-  let generated := NewNames.generate reserved $ UsedIn.term t in
-  option_map snd $ unshadow_acc generated (Map.set_union reserved $ Map.range generated) t.
-Arguments unshadow_reserve reserved t/.
+Definition unshadow_reserve_bindings cant_bind t :=
+  let generated := NewNames.generate cant_bind $ UsedIn.term t in
+  unshadow_acc generated (Map.set_union cant_bind $ Map.range generated) t.
+Arguments unshadow_reserve_bindings cant_bind t/.
+
+Definition unshadow_reserve cant_bind t := option_map snd $ unshadow_reserve_bindings cant_bind t.
+Arguments unshadow_reserve cant_bind t/.
 
 Definition unshadow := unshadow_reserve Map.empty.
 Arguments unshadow/ t.
 
 
 
-Lemma nodes_eq_acc {acc reserved t reserved' r} (E : unshadow_acc acc reserved t = Some (reserved', r))
+Lemma nodes_eq_acc {acc cant_bind t cant_bind' r} (E : unshadow_acc acc cant_bind t = Some (cant_bind', r))
   : Term.nodes r = Term.nodes t.
 Proof.
-  generalize dependent r. generalize dependent reserved'. generalize dependent reserved. generalize dependent acc.
+  generalize dependent r. generalize dependent cant_bind'. generalize dependent cant_bind. generalize dependent acc.
   induction t; intros; cbn in *.
   - invert E. reflexivity.
   - destruct Map.find; invert E. reflexivity.
@@ -80,9 +83,12 @@ Proof.
     apply Rename.pattern_nodes_eq in Ep as ->. reflexivity.
 Qed.
 
-Lemma nodes_eq_reserve {reserved t r} (E : unshadow_reserve reserved t = Some r)
+Lemma nodes_eq_reserve {cant_bind t r} (E : unshadow_reserve cant_bind t = Some r)
   : Term.nodes r = Term.nodes t.
-Proof. unfold unshadow_reserve in E. destruct unshadow_acc as [[] |] eqn:E'; invert E. eapply nodes_eq_acc. exact E'. Qed.
+Proof.
+  unfold unshadow_reserve in E. unfold unshadow_reserve_bindings in E.
+  destruct unshadow_acc as [[] |] eqn:E'; invert E. eapply nodes_eq_acc. exact E'.
+Qed.
 
 Lemma nodes_eq {t r} (E : unshadow t = Some r)
   : Term.nodes r = Term.nodes t.
@@ -94,8 +100,8 @@ Variant Equiv : option (Map.set * Term.term) -> _ -> Prop :=
   | ENone
       : Equiv None None
   | ESome
-      {reserved1 reserved2} (Ereserved : Map.Eq reserved1 reserved2) output
-      : Equiv (Some (reserved1, output)) (Some (reserved2, output))
+      {cant_bind1 cant_bind2} (Ecant_bind : Map.Eq cant_bind1 cant_bind2) output
+      : Equiv (Some (cant_bind1, output)) (Some (cant_bind2, output))
   .
 
 Lemma det_acc
@@ -111,56 +117,56 @@ Proof.
     + apply Ea in Y. apply Map.find_iff in Y. rewrite Y. constructor. exact Er.
     + destruct (Map.find_spec a2 name). { apply Ea in Y. apply N in Y as []. } constructor.
   - destruct (IHt1 _ _ Ea _ _ Er). { constructor. }
-    destruct (IHt2 _ _ Ea _ _ Ereserved); constructor; eassumption.
+    destruct (IHt2 _ _ Ea _ _ Ecant_bind); constructor; eassumption.
   - destruct (IHt1 _ _ Ea _ _ Er). { constructor. } eassert (Ea' : _); [| eassert (Er' : _); [| destruct (IHt2
-      (Map.overriding_add variable (NewNames.new_name reserved1 variable) a1)
-      (Map.overriding_add variable (NewNames.new_name reserved2 variable) a2) Ea'
-      (Map.overriding_add (NewNames.new_name reserved1 variable) tt reserved1)
-      (Map.overriding_add (NewNames.new_name reserved2 variable) tt reserved2) Er')]]. 3: { constructor. }
+      (Map.overriding_add variable (NewNames.new_name cant_bind1 variable) a1)
+      (Map.overriding_add variable (NewNames.new_name cant_bind2 variable) a2) Ea'
+      (Map.overriding_add (NewNames.new_name cant_bind1 variable) tt cant_bind1)
+      (Map.overriding_add (NewNames.new_name cant_bind2 variable) tt cant_bind2) Er')]]. 3: { constructor. }
     + split; intro F; apply Map.find_overriding_add; (apply Map.find_overriding_add in F as [[-> ->] | [N F]]; [left | right];
-      [split; [reflexivity | apply NewNames.new_name_det] | split; [exact N |]; apply Ea; exact F]); [| apply Map.eq_sym]; exact Ereserved.
+      [split; [reflexivity | apply NewNames.new_name_det] | split; [exact N |]; apply Ea; exact F]); [| apply Map.eq_sym]; exact Ecant_bind.
     + split; intro F; apply Map.find_overriding_add; (apply Map.find_overriding_add in F as [[-> ->] | [N F]]; [left | right];
-      [split; [| reflexivity]; apply NewNames.new_name_det | split; [| apply Ereserved; exact F];
-        intros ->; contradiction N; apply NewNames.new_name_det]); try exact Ereserved; apply Map.eq_sym; exact Ereserved.
-    + erewrite NewNames.new_name_det. { constructor. exact Ereserved0. } exact Ereserved.
+      [split; [| reflexivity]; apply NewNames.new_name_det | split; [| apply Ecant_bind; exact F];
+        intros ->; contradiction N; apply NewNames.new_name_det]); try exact Ecant_bind; apply Map.eq_sym; exact Ecant_bind.
+    + erewrite NewNames.new_name_det. { constructor. exact Ecant_bind0. } exact Ecant_bind.
   - destruct (IHt2 _ _ Ea _ _ Er). { constructor. } destruct Rename.pattern eqn:ER. 2: {
       destruct Rename.pattern eqn:ER2 at 1. 2: { constructor. }
       eapply (Rename.pattern_iff (NewNames.one_to_one_generate _ _)) in ER2.
       eapply (@Rename.pattern_eq _ (NewNames.one_to_one_generate _ _)) in ER2; try reflexivity.
       * eapply Rename.pattern_iff in ER2. rewrite ER2 in ER. discriminate ER.
-      * erewrite <- NewNames.generate_det. { apply Map.eq_refl. } { exact Ereserved. } apply Map.eq_refl. }
+      * erewrite <- NewNames.generate_det. { apply Map.eq_refl. } { exact Ecant_bind. } apply Map.eq_refl. }
     apply (Rename.pattern_iff (NewNames.one_to_one_generate _ _)) in ER.
     eapply (@Rename.pattern_eq _ (NewNames.one_to_one_generate _ _)) in ER; try reflexivity; [
       eapply Rename.pattern_iff in ER; rewrite ER; clear ER |
-      erewrite NewNames.generate_det; try apply Map.eq_refl; exact Ereserved].
+      erewrite NewNames.generate_det; try apply Map.eq_refl; exact Ecant_bind].
     eassert (Ea' : _); [| eassert (Er' : _); [| destruct (IHt1
       (Map.overriding_union (Map.fold (fun k _ acc => Map.overriding_add k (NewNames.new_name
-        (Map.overriding_union reserved1 $ Map.fold (fun _ v acc0 => Map.overriding_add v tt acc0) Map.empty acc) k) acc)
+        (Map.overriding_union cant_bind1 $ Map.fold (fun _ v acc0 => Map.overriding_add v tt acc0) Map.empty acc) k) acc)
         Map.empty (BoundIn.pattern pattern)) a1)
       (Map.overriding_union (Map.fold (fun k _ acc => Map.overriding_add k (NewNames.new_name
-        (Map.overriding_union reserved2 $ Map.fold (fun _ v acc0 => Map.overriding_add v tt acc0) Map.empty acc) k) acc)
+        (Map.overriding_union cant_bind2 $ Map.fold (fun _ v acc0 => Map.overriding_add v tt acc0) Map.empty acc) k) acc)
         Map.empty (BoundIn.pattern pattern)) a2) Ea'
       (Map.overriding_union (Map.fold (fun _ v acc => Map.overriding_add v tt acc) Map.empty
-        (Map.fold (fun k _ acc => Map.overriding_add k (NewNames.new_name (Map.overriding_union reserved1
+        (Map.fold (fun k _ acc => Map.overriding_add k (NewNames.new_name (Map.overriding_union cant_bind1
           (Map.fold (fun _ v acc0 => Map.overriding_add v tt acc0) Map.empty acc)) k) acc)
-          Map.empty (BoundIn.pattern pattern))) reserved1)
+          Map.empty (BoundIn.pattern pattern))) cant_bind1)
       (Map.overriding_union (Map.fold (fun _ v acc => Map.overriding_add v tt acc) Map.empty
-        (Map.fold (fun k _ acc => Map.overriding_add k (NewNames.new_name (Map.overriding_union reserved2
+        (Map.fold (fun k _ acc => Map.overriding_add k (NewNames.new_name (Map.overriding_union cant_bind2
           (Map.fold (fun _ v acc0 => Map.overriding_add v tt acc0) Map.empty acc)) k) acc)
-          Map.empty (BoundIn.pattern pattern))) reserved2) Er')]]. 3: { constructor. }
+          Map.empty (BoundIn.pattern pattern))) cant_bind2) Er')]]. 3: { constructor. }
     + assert (G := @NewNames.generate_det). cbn in G. erewrite G.
       * split; intro F; apply Map.bulk_overwrite_bulk_overwrite;
         (apply Map.bulk_overwrite_bulk_overwrite in F as [F | [N F]]; [left; exact F | right]);
         (split; [intro I; apply N; exact I |]; apply Ea; exact F).
-      * exact Ereserved.
+      * exact Ecant_bind.
       * apply Map.eq_refl.
     + assert (G := @NewNames.generate_det). cbn in G. erewrite G.
       * split; intro F; apply Map.bulk_overwrite_bulk_overwrite;
         (apply Map.bulk_overwrite_bulk_overwrite in F as [F | [N F]]; [left; exact F | right]);
-        (split; [intro I; apply N; exact I |]; apply Ereserved; exact F).
-      * exact Ereserved.
+        (split; [intro I; apply N; exact I |]; apply Ecant_bind; exact F).
+      * exact Ecant_bind.
       * apply Map.eq_refl.
-    + constructor. exact Ereserved0. }
+    + constructor. exact Ecant_bind0. }
   Unshelve.
   - apply NewNames.one_to_one_generate.
   - apply NewNames.one_to_one_generate.
@@ -171,7 +177,7 @@ Lemma det_reserve
   {t1 t2} (Et : t1 = t2)
   : unshadow_reserve r1 t1 = unshadow_reserve r2 t2.
 Proof.
-  unfold unshadow_reserve.
+  unfold unshadow_reserve. unfold unshadow_reserve_bindings.
   eassert (E1 : Map.Eq (NewNames.generate r1 $ UsedIn.term t1) (NewNames.generate r2 $ UsedIn.term t2)). {
     erewrite NewNames.generate_det. { apply Map.eq_refl. } { exact Er. } subst. apply Map.eq_refl. }
   eassert (E2 : Map.Eq
@@ -186,13 +192,13 @@ Qed.
 
 
 
-Lemma bindings {acc reserved term bindings renamed}
-  (E : unshadow_acc acc reserved term = Some (bindings, renamed))
-  (prev : forall x y (Fa : Map.Find acc x y), Map.In reserved y)
-  : Map.Reflect (fun x => BoundIn.Term renamed x \/ Map.In reserved x) bindings.
+Lemma bindings {acc cant_bind term bindings renamed}
+  (E : unshadow_acc acc cant_bind term = Some (bindings, renamed))
+  (prev : forall x y (Fa : Map.Find acc x y), Map.In cant_bind y)
+  : Map.Reflect (fun x => BoundIn.Term renamed x \/ Map.In cant_bind x) bindings.
 Proof.
   generalize dependent renamed. generalize dependent bindings.
-  generalize dependent reserved. generalize dependent acc. induction term; intros; simpl unshadow_acc in *.
+  generalize dependent cant_bind. generalize dependent acc. induction term; intros; simpl unshadow_acc in *.
   - invert E. split. { intro I. right. exact I. }
     intros [B | I]. { invert B. } exact I.
   - destruct (Map.find_spec acc name) as [name' F | N]; invert E.
@@ -244,41 +250,45 @@ Qed.
 
 
 
-Lemma wf_spec acc reserved t
-  : Reflect.Option
-    (fun _ => WellFormed.AllPatternsIn t /\ forall x (U : UsedIn.Term t x), Map.In acc x)
-    (unshadow_acc acc reserved t).
+Lemma wf_patterns_spec_acc acc cant_bind t
+  : Reflect.Option (fun '(cant_bind', t') =>
+      WellFormed.AllPatternsIn t /\
+      WellFormed.AllPatternsIn t' /\
+      forall x (U : UsedIn.Term t x), Map.In acc x
+    ) $ unshadow_acc acc cant_bind t.
 Proof.
-  generalize dependent reserved. generalize dependent acc. induction t; intros; cbn in *.
-  - constructor. split; intros. { constructor. } invert U.
+  generalize dependent cant_bind. generalize dependent acc. induction t; intros; cbn in *.
+  - constructor. split. { constructor. } split. { constructor. } intros. invert U.
   - destruct (Map.find_spec acc name); constructor.
-    + split; intros. { constructor. } invert U. eexists. exact Y.
-    + intros _ [_ C]. edestruct C. { constructor. } apply N in H as [].
-  - destruct (IHt1 acc reserved) as [[r1 t1'] [WF1 IH1] |]. 2: {
-      constructor. intros pair [WF C]. invert WF. apply N. { exact pair. }
-      split. { exact APf. } intros. apply C. apply UsedIn.ApF. exact U. }
-    destruct (IHt2 acc r1) as [[r2 t2'] [WF2 IH2] |]; constructor.
-    + constructor. { constructor; assumption. } intros. invert U; [apply IH1 | apply IH2]; assumption.
-    + intros pair [WF C]. invert WF. apply N. { exact pair. }
-      split. { exact APa. } intros. apply C. apply UsedIn.ApA. exact U.
-  - destruct (IHt1 acc reserved) as [[r1 t1'] [WF1 IH1] |]. 2: {
-      constructor. intros pair [WF C]. invert WF. apply N. { exact pair. }
-      split. { exact APt. } intros. apply C. apply UsedIn.FoT. exact U. }
+    + split; intros. { constructor. } split. { constructor. } intros. invert U. eexists. exact Y.
+    + intros [cant_bind' t'] [WF [WF' C]]. edestruct C. { constructor. } apply N in H as [].
+  - destruct (IHt1 acc cant_bind) as [[r1 t1'] [WF1 [WF1' IH1]] |]. 2: {
+      constructor. intros [cant_bind' t'] [WF [WF' C]]. invert WF. eapply (N (cant_bind', t')).
+      split. { exact APf. } split. { exact WF'. } intros. apply C. apply UsedIn.ApF. exact U. }
+    destruct (IHt2 acc r1) as [[r2 t2'] [WF2 [WF2' IH2]] |]; constructor.
+    + split. { constructor; assumption. } split. { constructor. { exact WF1'. } exact WF2'. }
+      intros. invert U; [apply IH1 | apply IH2]; assumption.
+    + intros [cant_bind' t'] [WF [WF' C]]. invert WF. apply (N (cant_bind', t')).
+      split. { exact APa. } split. { exact WF'. } intros. apply C. apply UsedIn.ApA. exact U.
+  - destruct (IHt1 acc cant_bind) as [[r1 t1'] [WF1 [WF1' IH1]] |]. 2: {
+      constructor. intros [cant_bind' t'] [WF [WF' C]]. invert WF. apply (N (cant_bind', t')).
+      split. { exact APt. } split. { exact WF'. } intros. apply C. apply UsedIn.FoT. exact U. }
     destruct (IHt2 (Map.overriding_add variable (NewNames.new_name r1 variable) acc)
-      (Map.overriding_add (NewNames.new_name r1 variable) tt r1)) as [[r2 t2'] [WF2 IH2] |]; constructor.
-    + split. { constructor; assumption. } intros. invert U. { apply IH1. exact used_in_type. }
+      (Map.overriding_add (NewNames.new_name r1 variable) tt r1)) as [[r2 t2'] [WF2 [WF2' IH2]] |]; constructor.
+    + split. { constructor; assumption. } split. { constructor. { exact WF1'. } exact WF2'. }
+      intros. invert U. { apply IH1. exact used_in_type. }
       apply IH2 in used_in_body. apply Map.in_overriding_add in used_in_body as [-> | I]. 2: { exact I. }
       contradiction not_shadowed. reflexivity.
-    + intros pair [WF C]. invert WF. apply N. { exact pair. }
-      split. { exact APb. } intros. apply Map.in_overriding_add.
+    + intros [cant_bind' t'] [WF [WF' C]]. invert WF. apply (N (cant_bind', t')).
+      split. { exact APb. } split. { exact WF'. } intros. apply Map.in_overriding_add.
       destruct (String.eqb_spec x variable); [left | right]. { assumption. } apply C. apply UsedIn.FoB; assumption.
-  - destruct (IHt2 acc reserved) as [[r2 t2'] [WF2 IH2] |]. 2: {
-      constructor. intros pair [WF C]. invert WF. apply N. { exact pair. }
-      split. { exact APo. } intros. apply C. apply UsedIn.CaO. exact U. }
+  - destruct (IHt2 acc cant_bind) as [[r2 t2'] [WF2 [WF2' IH2]] |]. 2: {
+      constructor. intros [cant_bind' t'] [WF [WF' C]]. invert WF. apply (N (cant_bind', t')).
+      split. { exact APo. } split. { exact WF'. } intros. apply C. apply UsedIn.CaO. exact U. }
     destruct (@Rename.pattern_spec (Map.fold (fun k _ acc' => Map.overriding_add k (NewNames.new_name
       (Map.overriding_union r2 (Map.fold (fun _ v acc'' => Map.overriding_add v tt acc'') Map.empty acc'))
       k) acc') Map.empty (BoundIn.pattern pattern)) (NewNames.one_to_one_generate _ _) pattern). 2: {
-      constructor. intros pair [WF C]. invert WF. eassert (RC : Rename.CompatiblePattern _ _). 2: {
+      constructor. intros [cant_bind' t'] [WF [WF' C]]. invert WF. eassert (RC : Rename.CompatiblePattern _ _). 2: {
         apply Rename.pattern_iff_compatible in RC as [O2O [renamed R]].
         eapply Rename.pattern_eq in R; try reflexivity. { apply N in R as []. } apply Map.eq_refl. }
       invert WFp; constructor. { apply NewNames.one_to_one_generate. } {
@@ -293,25 +303,52 @@ Proof.
       (Map.overriding_union (Map.fold (fun _ v acc' => Map.overriding_add v tt acc') Map.empty (Map.fold
         (fun k _ acc' => Map.overriding_add k (NewNames.new_name (Map.overriding_union r2 (Map.fold
           (fun _ v acc'' => Map.overriding_add v tt acc'') Map.empty acc')) k) acc')
-        Map.empty (BoundIn.pattern pattern))) r2)) as [[r1 t1'] [WF1 IH1] |]; constructor.
+        Map.empty (BoundIn.pattern pattern))) r2)) as [[r1 t1'] [WF1 [WF1' IH1]] |]; constructor.
     + constructor. { constructor; try assumption. invert RC; constructor. invert C; constructor; apply CS. }
+      split. { constructor. 2: { exact WF1'. } 2: { exact WF2'. } invert Y; constructor.
+        invert rename_move_or_reference; constructor; eapply Rename.wf_strict; exact rename_strict. }
       intros z U. invert U. 2: { apply IH2. exact used_in_another_case. } apply IH1 in used_in_body.
       apply Map.in_overriding_union in used_in_body as [I | I]. 2: { exact I. }
       apply NewNames.in_generate in I. apply BoundIn.pattern_iff in I. apply not_shadowed in I as [].
-    + intros pair [WF C]. invert WF. apply N. { exact pair. } split. { exact APb. } intros.
+    + intros [cant_bind' t'] [WF [WF' C]]. invert WF. apply (N (cant_bind', t')).
+      split. { exact APb. } split. { exact WF'. } intros.
       apply Map.in_overriding_union. destruct (BoundIn.pattern_spec pattern x0); [left | right].
       * apply NewNames.in_generate. apply BoundIn.pattern_iff. exact Y0.
       * apply C. apply UsedIn.CaB; assumption.
 Qed.
 
-Lemma disjoint_used {acc reserved term reserved' renamed}
-  (E : unshadow_acc acc reserved term = Some (reserved', renamed))
-  (prev : forall x y (Fa : Map.Find acc x y), Map.In reserved y)
-  {y} (I : Map.In reserved y) (U : UsedIn.Term renamed y)
+Lemma wf_patterns_spec_bindings cant_bind t
+  : Reflect.Option (fun '(cant_bind', t') =>
+      WellFormed.AllPatternsIn t /\ WellFormed.AllPatternsIn t'
+    ) $ unshadow_reserve_bindings cant_bind t.
+Proof.
+  unfold unshadow_reserve. unfold unshadow_reserve_bindings.
+  destruct (wf_patterns_spec_acc (NewNames.generate cant_bind $ UsedIn.term t)
+    (Map.set_union cant_bind $ Map.range $ NewNames.generate cant_bind $ UsedIn.term t) t) as [[domain' renamed] |]; cbn; constructor.
+  - destruct Y as [WF [WF' AU]]. split. { exact WF. } exact WF'.
+  - intros [cant_bind' t'] [WF WF']. apply (N (cant_bind', t')). split. { exact WF. }
+    split. { exact WF'. } intros. apply NewNames.in_generate. apply UsedIn.term_iff. exact U.
+Qed.
+
+Lemma wf_patterns_spec domain t
+  : Reflect.Option (fun t' =>
+      WellFormed.AllPatternsIn t /\ WellFormed.AllPatternsIn t'
+    ) $ unshadow_reserve domain t.
+Proof.
+  unfold unshadow_reserve. destruct (wf_patterns_spec_bindings domain t) as [[cant_bind' t'] |];
+  constructor. { exact Y. } intro. exact (N (Map.empty, x)).
+Qed.
+
+
+
+Lemma disjoint_used {acc cant_bind term cant_bind' renamed}
+  (E : unshadow_acc acc cant_bind term = Some (cant_bind', renamed))
+  (prev : forall x y (Fa : Map.Find acc x y), Map.In cant_bind y)
+  {y} (I : Map.In cant_bind y) (U : UsedIn.Term renamed y)
   : exists x, Map.Find acc x y.
 Proof.
-  generalize dependent y. generalize dependent renamed. generalize dependent reserved'.
-  generalize dependent reserved. generalize dependent acc. induction term; intros; cbn in *.
+  generalize dependent y. generalize dependent renamed. generalize dependent cant_bind'.
+  generalize dependent cant_bind. generalize dependent acc. induction term; intros; cbn in *.
   - invert E. invert U.
   - destruct (Map.find_spec acc name); invert E. invert U. eexists. exact Y.
   - destruct unshadow_acc as [[r1 t1] |] eqn:E1 in E. 2: { discriminate E. }
@@ -344,14 +381,14 @@ Proof.
     + apply Map.in_overriding_union. right. eapply bindings. { exact E2. } { exact prev. } right. exact I.
 Qed.
 
-Lemma disjoint_bound {acc reserved term reserved' renamed}
-  (E : unshadow_acc acc reserved term = Some (reserved', renamed))
-  (prev : forall x y (Fa : Map.Find acc x y), Map.In reserved y)
-  {x} (I : Map.In reserved x) (B : BoundIn.Term renamed x)
+Lemma disjoint_bound {acc cant_bind term cant_bind' renamed}
+  (E : unshadow_acc acc cant_bind term = Some (cant_bind', renamed))
+  (prev : forall x y (Fa : Map.Find acc x y), Map.In cant_bind y)
+  {x} (I : Map.In cant_bind x) (B : BoundIn.Term renamed x)
   : False.
 Proof.
-  generalize dependent x. generalize dependent renamed. generalize dependent reserved'.
-  generalize dependent reserved. generalize dependent acc. induction term; intros; cbn in *.
+  generalize dependent x. generalize dependent renamed. generalize dependent cant_bind'.
+  generalize dependent cant_bind. generalize dependent acc. induction term; intros; cbn in *.
   - invert E. invert B.
   - destruct (Map.find_spec acc name); invert E. invert B.
   - destruct unshadow_acc as [[r1 t1] |] eqn:E1 in E. 2: { discriminate E. }
@@ -383,14 +420,14 @@ Proof.
     + eapply IHterm2. { exact prev. } { exact E2. } { exact I. } exact bound_in_another_case.
 Qed.
 
-Lemma used_reserved {acc reserved term reserved' renamed}
-  (E : unshadow_acc acc reserved term = Some (reserved', renamed))
-  (prev : forall x y (Fa : Map.Find acc x y), Map.In reserved y)
+Lemma used_cant_bind {acc cant_bind term cant_bind' renamed}
+  (E : unshadow_acc acc cant_bind term = Some (cant_bind', renamed))
+  (prev : forall x y (Fa : Map.Find acc x y), Map.In cant_bind y)
   {x} (U : UsedIn.Term renamed x)
-  : Map.In reserved' x.
+  : Map.In cant_bind' x.
 Proof.
-  generalize dependent x. generalize dependent renamed. generalize dependent reserved'.
-  generalize dependent reserved. generalize dependent acc. induction term; intros; cbn in *.
+  generalize dependent x. generalize dependent renamed. generalize dependent cant_bind'.
+  generalize dependent cant_bind. generalize dependent acc. induction term; intros; cbn in *.
   - invert E. invert U.
   - destruct (Map.find_spec acc name); invert E. invert U. eapply prev. exact Y.
   - destruct unshadow_acc as [[r1 t1] |] eqn:E1 in E. 2: { discriminate E. }
@@ -432,116 +469,1244 @@ Qed.
 
 
 
-Inductive Unshadowed : Term.term -> Prop :=
+(* This relation asks whether another specified relation holds of any root and its children, anywhere in the tree.
+ * There are two versions: lateral, in which all roots are tested symmetrically, and
+ * non-lateral, in which a relation may depend on differing contexts between children (specifically, `For` and `Cas` nodes). *)
+Inductive Anywhere (Lateral : Prop)
+  (P : forall (bindings : String.string -> Prop) (aux deep : Term.term), Prop)
+  : Term.term -> Prop :=
+  | APAF (lateral : Lateral) {function argument} (here : P (fun _ => False) function argument)
+      : Anywhere Lateral P $ Term.App function argument
+  | APAA (lateral : Lateral) {function argument} (here : P (fun _ => False) argument function)
+      : Anywhere Lateral P $ Term.App function argument
+  | APFT {variable type body} (here : P (eq variable) type body)
+      : Anywhere Lateral P $ Term.For variable type body
+  | APFB (lateral : Lateral) {variable type body} (here : P (eq variable) body type)
+      : Anywhere Lateral P $ Term.For variable type body
+  | APCB (lateral : Lateral) {pattern body_if_match other_cases} (here : P (BoundIn.Pattern pattern) body_if_match other_cases)
+      : Anywhere Lateral P $ Term.Cas pattern body_if_match other_cases
+  | APCO {pattern body_if_match other_cases} (here : P (BoundIn.Pattern pattern) other_cases body_if_match)
+      : Anywhere Lateral P $ Term.Cas pattern body_if_match other_cases
+  | ARAF {function} (R : Anywhere Lateral P function) argument
+      : Anywhere Lateral P $ Term.App function argument
+  | ARAA {argument} (R : Anywhere Lateral P argument) function
+      : Anywhere Lateral P $ Term.App function argument
+  | ARFT {type} (R : Anywhere Lateral P type) variable body
+      : Anywhere Lateral P $ Term.For variable type body
+  | ARFB {body} (R : Anywhere Lateral P body) variable type
+      : Anywhere Lateral P $ Term.For variable type body
+  | ARCB {body_if_match} (R : Anywhere Lateral P body_if_match) pattern other_cases
+      : Anywhere Lateral P $ Term.Cas pattern body_if_match other_cases
+  | ARCO {other_cases} (R : Anywhere Lateral P other_cases) pattern body_if_match
+      : Anywhere Lateral P $ Term.Cas pattern body_if_match other_cases
+  .
+Arguments Anywhere Lateral P t.
+
+(* If a variable is bound at the root of a subtree and then bound again in that subtree: *)
+Definition HasShadow := Anywhere True $ fun Bound child _ => exists x, Bound x /\ BoundIn.Term child x.
+
+(* If a variable is bound in one subtree of the AST and used in an adjacent subtree: *)
+(* (name from Einstein's "spooky action at a distance" remark) *)
+Definition Spooky := Anywhere True $ fun _ child1 child2 => exists x, UsedIn.Term child1 x /\ BoundIn.Term child2 x.
+
+(* If a variable is bound in both children, separately: *)
+Definition Parallel := Anywhere True $ fun _ child1 child2 => exists x, BoundIn.Term child1 x /\ BoundIn.Term child2 x.
+
+(* If a variable is bound and then used immediately in a child,
+ * but the wrong child (e.g. `forall x : x, ...` or `case x => { ... } else x`): *)
+Definition LateralScope := Anywhere False $ fun Bound cant_use_bindings _ => exists x, Bound x /\ UsedIn.Term cant_use_bindings x.
+
+
+
+Definition WellFormedNeg t : Prop := (~HasShadow t) /\ (~Spooky t) /\ (~Parallel t) /\ (~LateralScope t).
+Arguments WellFormedNeg t/.
+
+Definition WellFormedNegInAcc (cant_bind context : Map.set) t : Prop :=
+  WellFormedNeg t /\ forall x, (
+    (forall (B : BoundIn.Term t x) (I : Map.In cant_bind x), False) /\
+    (forall (U : UsedIn.Term t x), Map.In context x)).
+Arguments WellFormedNegInAcc cant_bind context t/.
+
+Definition WellFormedNegIn context := WellFormedNegInAcc context context.
+Arguments WellFormedNegIn context t/.
+
+Definition bind {A B C} (f : A -> B -> option C) (x : option (A * B)) :=
+  match x with None => None | Some (bound, used) => f bound used end.
+Arguments bind {A B C} f x/.
+
+Fixpoint well_formed_in_acc cant_bind context t :=
+  match t with
+  | Term.Ctr _ => Some (Map.empty, Map.empty)
+  | Term.Var name _ => if Map.in_ context name then Some (Map.empty, Map.singleton name tt) else None
+  | Term.App function argument =>
+      bind (fun bound_in_function used_in_function =>
+        bind (fun bound_in_argument used_in_argument =>
+          if Map.disjoint bound_in_function bound_in_argument then
+            if Map.disjoint bound_in_function used_in_argument then
+              if Map.disjoint bound_in_argument used_in_function then Some (
+                Map.set_union bound_in_function bound_in_argument,
+                Map.set_union used_in_function used_in_argument)
+              else None
+            else None
+          else None
+        ) (well_formed_in_acc cant_bind context argument)
+      ) (well_formed_in_acc cant_bind context function)
+  | Term.For variable type body =>
+      bind (fun bound_in_type used_in_type =>
+        let cant_bind_in_body_without_bindings := Map.set_union cant_bind $ Map.set_union bound_in_type used_in_type in
+        if Map.in_ cant_bind_in_body_without_bindings variable then None else
+        let cant_bind_in_body := Map.set_add variable cant_bind_in_body_without_bindings in
+        let context_in_body := Map.set_add variable context in
+        bind (fun bound_in_body used_in_body =>
+          if Map.disjoint bound_in_type bound_in_body then
+            if Map.disjoint bound_in_type used_in_body then
+              if Map.disjoint bound_in_body used_in_type then Some (
+                Map.set_add variable $ Map.set_union bound_in_type bound_in_body,
+                Map.set_union used_in_type $ Map.remove variable used_in_body)
+              else None
+            else None
+          else None
+        ) (well_formed_in_acc cant_bind_in_body context_in_body body)
+      ) (well_formed_in_acc cant_bind context type)
+  | Term.Cas pattern body_if_match other_cases =>
+      bind (fun bound_in_other_cases used_in_other_cases =>
+        let cant_bind_in_body_without_bindings := Map.set_union cant_bind $ Map.set_union bound_in_other_cases used_in_other_cases in
+        let bound_in_pattern := BoundIn.pattern pattern in
+        if Map.disjoint cant_bind_in_body_without_bindings bound_in_pattern then
+          let cant_bind_in_body_if_match := Map.set_union bound_in_pattern cant_bind_in_body_without_bindings in
+          let context_in_body_if_match := Map.set_union bound_in_pattern context in
+          bind (fun bound_in_body_if_match used_in_body_if_match =>
+            if Map.disjoint bound_in_other_cases bound_in_body_if_match then
+              if Map.disjoint bound_in_other_cases used_in_body_if_match then
+                if Map.disjoint bound_in_body_if_match used_in_other_cases then Some (
+                  Map.set_union bound_in_pattern $ Map.set_union bound_in_other_cases bound_in_body_if_match,
+                  Map.set_union used_in_other_cases $ Map.minus used_in_body_if_match bound_in_pattern)
+                else None
+              else None
+            else None
+          ) (well_formed_in_acc cant_bind_in_body_if_match context_in_body_if_match body_if_match)
+        else None
+      ) (well_formed_in_acc cant_bind context other_cases)
+  end.
+
+Definition well_formed_in context t :=
+  match well_formed_in_acc context context t with
+  | None => false
+  | Some _ => true
+  end.
+
+Lemma bound_used {cant_bind context t bound used} (E : well_formed_in_acc cant_bind context t = Some (bound, used))
+  : Map.Reflect (BoundIn.Term t) bound /\ Map.Reflect (UsedIn.Term t) used.
+Proof.
+  generalize dependent used. generalize dependent bound. generalize dependent context. generalize dependent cant_bind.
+  induction t; intros; cbn in *.
+  - invert E. split; intro x.
+    + split. { intro I. apply Map.empty_empty in I as []. } intro B. invert B.
+    + split. { intro I. apply Map.empty_empty in I as []. } intro U. invert U.
+  - destruct (Map.in_spec context name); invert E. split; intro x.
+    + split. { intro I. apply Map.empty_empty in I as []. } intro B. invert B.
+    + split. { intro I. apply Map.in_singleton in I as ->. constructor. } intro U. invert U. apply Map.in_singleton. reflexivity.
+  - destruct well_formed_in_acc as [[b1 u1] |] eqn:E1 in E. 2: { discriminate E. }
+    destruct well_formed_in_acc as [[b2 u2] |] eqn:E2 in E. 2: { discriminate E. }
+    specialize (IHt1 _ _ _ _ E1) as [B1 U1]. specialize (IHt2 _ _ _ _ E2) as [B2 U2].
+    destruct Map.disjoint eqn:D1 in E. 2: { discriminate E. }
+    destruct Map.disjoint eqn:D2 in E. 2: { discriminate E. }
+    destruct Map.disjoint eqn:D3 in E; invert E. split; intro x; rewrite Map.in_overriding_union.
+    + split.
+      * intros [I | I]; [apply BoundIn.TApF | apply BoundIn.TApA]; [apply B1 | apply B2]; exact I.
+      * intro B. invert B; [left | right]; [apply B1 | apply B2]; assumption.
+    + split.
+      * intros [I | I]; [apply UsedIn.ApF | apply UsedIn.ApA]; [apply U1 | apply U2]; exact I.
+      * intro U. invert U; [left | right]; [apply U1 | apply U2]; assumption.
+  - destruct well_formed_in_acc as [[b1 u1] |] eqn:E1 in E. 2: { discriminate E. }
+    destruct (Map.in_spec (Map.overriding_union cant_bind $ Map.overriding_union b1 u1) variable). { discriminate E. }
+    destruct well_formed_in_acc as [[b2 u2] |] eqn:E2 in E. 2: { discriminate E. }
+    specialize (IHt1 _ _ _ _ E1) as [B1 U1]. specialize (IHt2 _ _ _ _ E2) as [B2 U2].
+    destruct Map.disjoint eqn:D1 in E. 2: { discriminate E. }
+    destruct Map.disjoint eqn:D2 in E. 2: { discriminate E. }
+    destruct Map.disjoint eqn:D3 in E; invert E. split; intro x.
+    + rewrite Map.in_overriding_add. rewrite Map.in_overriding_union. split.
+      * intros [-> | [I | I]]; [apply BoundIn.TFoV | apply BoundIn.TFoT | apply BoundIn.TFoB]; [apply B1 | apply B2]; exact I.
+      * intro B. invert B; [left; reflexivity | |]; right; [left | right]; [apply B1 | apply B2]; assumption.
+    + rewrite Map.in_overriding_union. rewrite (Map.in_remove_if_present $ Map.remove_if_present_remove _ _). split.
+      * intros [I | [Nx I]]; [apply UsedIn.FoT | apply UsedIn.FoB]; [apply U1 | exact Nx | apply U2]; exact I.
+      * intro U. invert U; [left | right]; [| split; [exact not_shadowed |]]; [apply U1 | apply U2]; assumption.
+  - destruct well_formed_in_acc as [[b2 u2] |] eqn:E2 in E. 2: { discriminate E. }
+    destruct Map.disjoint eqn:D1 in E. 2: { discriminate E. }
+    destruct well_formed_in_acc as [[b1 u1] |] eqn:E1 in E. 2: { discriminate E. }
+    specialize (IHt1 _ _ _ _ E1) as [B1 U1]. specialize (IHt2 _ _ _ _ E2) as [B2 U2].
+    destruct Map.disjoint eqn:D2 in E. 2: { discriminate E. }
+    destruct Map.disjoint eqn:D3 in E. 2: { discriminate E. }
+    destruct Map.disjoint eqn:D4 in E; invert E. split; intro x; repeat rewrite Map.in_overriding_union.
+    + split.
+      * intros [I | [I | I]]; [apply BoundIn.TCaP; apply BoundIn.pattern_iff; exact I | |];
+        [apply BoundIn.TCaO | apply BoundIn.TCaB]; [apply B2 | apply B1]; try exact I.
+      * intro B. invert B; [left; apply BoundIn.pattern_iff; exact bound_in_pattern | |];
+        right; [right | left]; [apply B1 | apply B2]; assumption.
+    + rewrite Map.in_minus. split.
+      * intros [I | [I N]]; [apply UsedIn.CaO | apply UsedIn.CaB]; [apply U2 | | apply U1]; try exact I.
+        intro B. apply N. apply BoundIn.pattern_iff. exact B.
+      * intro U. invert U; [right | left]; [split |]; [apply U1 | | apply U2]; try assumption.
+        intro B. apply not_shadowed. apply BoundIn.pattern_iff. exact B.
+Qed.
+
+Lemma well_formed_in_acc_spec
+  {t context} (no_free_vars : forall x (U : UsedIn.Term t x), Map.In context x)
+  {cant_bind} (cant_bind_context : forall x (I : Map.In context x), Map.In cant_bind x)
+  : Reflect.Option (fun _ => WellFormedNegInAcc cant_bind context t) $
+    well_formed_in_acc cant_bind context t.
+Proof.
+  generalize dependent cant_bind. generalize dependent context. induction t; intros; cbn in *.
+  - constructor. split. { repeat split; intro C; invert C. } split; intros. { invert B. } invert U.
+  - destruct (Map.in_spec context name); constructor.
+    + split. { repeat split; intro C; invert C. } split; intros. { invert B. } invert U. exact Y.
+    + eintros _ [_ [_ C]]. apply N in C as []. constructor.
+  - eassert (no_free_vars_1 : _); [| specialize (IHt1 context no_free_vars_1 cant_bind cant_bind_context)]. {
+      intros. apply no_free_vars. apply UsedIn.ApF. exact U. }
+    destruct well_formed_in_acc as [[b1 u1] |] eqn:E1 in IHt1; rewrite E1; invert IHt1. 2: {
+      constructor. intros pair [[NH [NS [NP NL]]] C]. apply (N pair). split. 2: { intro x. specialize (C x) as [C1 C2].
+        split; intros; [apply C1 | apply C2]. { apply BoundIn.TApF. exact B. } { exact I. } apply UsedIn.ApF. exact U. }
+      repeat split; intro; [apply NH | apply NS | apply NP | apply NL]; apply ARAF; assumption. }
+    eassert (no_free_vars_2 : _); [| specialize (IHt2 context no_free_vars_2 cant_bind cant_bind_context)]. {
+      intros. apply no_free_vars. apply UsedIn.ApA. exact U. }
+    destruct well_formed_in_acc as [[b2 u2] |] eqn:E2 in IHt2; rewrite E2; invert IHt2. 2: {
+      constructor. intros pair [[NH [NS [NP NL]]] C]. apply (N pair). split. 2: { intro x. specialize (C x) as [C1 C2].
+        split; intros; [apply C1 | apply C2]. { apply BoundIn.TApA. exact B. } { exact I. } apply UsedIn.ApA. exact U. }
+      repeat split; intro; [apply NH | apply NS | apply NP | apply NL]; apply ARAA; assumption. }
+    destruct (bound_used E1) as [B1 U1]. destruct (bound_used E2) as [B2 U2]. destruct (Map.disjoint_spec b1 b2). 2: {
+      constructor. intros _ [[_ [_ [C _]]] _]. apply C. apply APAF. { constructor. }
+      apply Map.not_disjoint_exists in N as [x [C1 C2]]. exists x. split; [apply B1 | apply B2]; assumption. }
+    destruct (Map.disjoint_spec b1 u2). 2: {
+      constructor. intros _ [[_ [C [_ _]]] _]. apply C. apply APAA. { constructor. }
+      apply Map.not_disjoint_exists in N as [x [C1 C2]]. exists x. split; [apply U2 | apply B1]; assumption. }
+    destruct (Map.disjoint_spec b2 u1); constructor. 2: {
+      intros _ [[_ [C [_ _]]] _]. apply C. apply APAF. { constructor. }
+      apply Map.not_disjoint_exists in N as [x [C1 C2]]. exists x. split; [apply U1 | apply B2]; assumption. }
+    split.
+    + repeat split; intro C; invert C; try solve [destruct here as [_ [[]]]];
+      try solve [apply Y in R as []]; try solve [apply Y0 in R as []].
+      * destruct here as [x [U1' B2']]. apply (Y3 x); [apply B2 | apply U1]; assumption.
+      * destruct here as [x [U2' B1']]. apply (Y2 x); [apply B1 | apply U2]; assumption.
+      * destruct here as [x [B1' B2']]. apply (Y1 x); [apply B1 | apply B2]; assumption.
+      * destruct here as [x [B2' B1']]. apply (Y1 x); [apply B1 | apply B2]; assumption.
+    + destruct Y as [_ H1]. destruct Y0 as [_ H2]. split; intros.
+      * invert B; [eapply H1 | eapply H2]; eassumption.
+      * invert U; [apply H1 | apply H2]; assumption.
+  - eassert (no_free_vars_1 : _); [| specialize (IHt1 context no_free_vars_1 cant_bind cant_bind_context)]. {
+      intros. apply no_free_vars. apply UsedIn.FoT. exact U. }
+    destruct well_formed_in_acc as [[b1 u1] |] eqn:E1 in IHt1; rewrite E1; invert IHt1. 2: {
+      constructor. intros pair [[NH [NS [NP NL]]] C]. apply (N pair). split. 2: { intro x. specialize (C x) as [C1 C2].
+        split; intros; [apply C1 | apply C2]. { apply BoundIn.TFoT. exact B. } { exact I. } apply UsedIn.FoT. exact U. }
+      repeat split; intro; [apply NH | apply NS | apply NP | apply NL]; apply ARFT; assumption. } destruct (bound_used E1) as [B1 U1].
+    destruct (Map.in_spec (Map.overriding_union cant_bind $ Map.overriding_union b1 u1) variable). { constructor.
+      intros _ [[NH [NS [NP NL]]] C]. apply Map.in_overriding_union in Y0 as [I | I]. { eapply C. { apply BoundIn.TFoV. } exact I. }
+      apply Map.in_overriding_union in I as [I | I]; [apply B1 in I as B | apply U1 in I as U].
+      * apply NH. apply APFT. exists variable. split. { reflexivity. } exact B.
+      * apply NL. apply APFT. exists variable. split. { reflexivity. } exact U. }
+    eassert (no_free_vars_2 : _); [| specialize (IHt2 (Map.overriding_add variable tt context)
+      no_free_vars_2 (Map.overriding_add variable tt $ Map.overriding_union cant_bind $ Map.overriding_union b1 u1))]. {
+      intros. apply Map.in_overriding_add. destruct (String.eqb_spec x variable); [left | right]. { exact e. }
+      apply no_free_vars. apply UsedIn.FoB. { exact n. } exact U. }
+    eassert (cant_bind_context' : _); [| specialize (IHt2 cant_bind_context')]. {
+      intro x. repeat rewrite Map.in_overriding_add. destruct (String.eqb_spec x variable); [left | right]. { exact e. }
+      destruct I as [E | I]. { apply n in E as []. } repeat rewrite Map.in_overriding_union. left. apply cant_bind_context. exact I. }
+    destruct well_formed_in_acc as [[b2 u2] |] eqn:E2 in IHt2; rewrite E2 in *; invert IHt2. 2: {
+      constructor. intros pair [[NH [NS [NP NL]]] C]. apply (N0 pair). split. {
+        repeat split; intro NA; [apply NH | apply NS | apply NP | apply NL]; apply ARFB; exact NA. }
+      intro x. specialize (C x) as [C1 C2]. split.
+      * intros B I. apply Map.in_overriding_add in I as [-> | I]. {
+          apply NH. apply APFB. { constructor. } exists variable. split. { reflexivity. } exact B. }
+        apply Map.in_overriding_union in I as [I | I]. { eapply C1. 2: { exact I. } apply BoundIn.TFoB. exact B. }
+        apply Map.in_overriding_union in I as [I | I]. { apply B1 in I. eapply NP. apply APFT. exists x. split; assumption. }
+        apply U1 in I. apply NS. apply APFT. exists x. split. { exact I. } exact B.
+      * intro U. apply Map.in_overriding_add. destruct (String.eqb_spec x variable); [left | right]. { exact e. }
+        apply C2. apply UsedIn.FoB. { exact n. } exact U. } destruct (bound_used E2) as [B2 U2].
+    destruct (Map.disjoint_spec b1 b2). 2: {
+      constructor. intros _ [[_ [_ [C _]]] _]. apply C. apply APFT.
+      apply Map.not_disjoint_exists in N0 as [x [C1 C2]]. exists x. split; [apply B1 | apply B2]; assumption. }
+    destruct (Map.disjoint_spec b1 u2). 2: {
+      constructor. intros _ [[_ [C [_ _]]] _]. apply C. apply APFB. { constructor. }
+      apply Map.not_disjoint_exists in N0 as [x [C1 C2]]. exists x. split; [apply U2 | apply B1]; assumption. }
+    destruct (Map.disjoint_spec b2 u1); constructor. 2: {
+      intros _ [[_ [C [_ _]]] _]. apply C. apply APFT.
+      apply Map.not_disjoint_exists in N0 as [x [C1 C2]]. exists x. split; [apply U1 | apply B2]; assumption. }
+    split.
+    + repeat split; intro C; invert C; try solve [apply Y in R as []]; try solve [apply Y0 in R as []];
+      destruct Y as [[NH1 [NS1 [NP1 NL1]]] C1]; destruct Y0 as [[NH2 [NS2 [NP2 NL2]]] C2].
+      * destruct here as [x [<- B]]. apply N. apply Map.in_overriding_union. right.
+        apply Map.in_overriding_union. left. apply B1. exact B.
+      * destruct here as [x [<- B]]. eapply C2. { exact B. } apply Map.in_overriding_add. left. reflexivity.
+      * destruct here as [x [U B]]. eapply (Y3 x); [apply B2 | apply U1]; assumption.
+      * destruct here as [x [U B]]. eapply (Y2 x); [apply B1 | apply U2]; assumption.
+      * destruct here as [x [B1' B2']]. eapply (Y1 x); [apply B1 | apply B2]; assumption.
+      * destruct here as [x [B2' B1']]. eapply (Y1 x); [apply B1 | apply B2]; assumption.
+      * destruct here as [x [<- U]]. apply N. apply Map.in_overriding_union. right.
+        apply Map.in_overriding_union. right. apply U1. exact U.
+      * destruct lateral as [].
+    + destruct Y as [[NH1 [NS1 [NP1 NL1]]] C1]. destruct Y0 as [[NH2 [NS2 [NP2 NL2]]] C2]. split; intros.
+      * invert B. { apply N. apply Map.in_overriding_union. left. exact I. } { apply (C1 x); assumption. }
+        apply (C2 x). { exact bound_in_body. } apply Map.in_overriding_add. right. apply Map.in_overriding_union. left. exact I.
+      * invert U. { apply no_free_vars_1. exact used_in_type. } apply no_free_vars_2 in used_in_body.
+        apply Map.in_overriding_add in used_in_body as [E | U]. { apply not_shadowed in E as []. } exact U.
+  - eassert (no_free_vars_2 : _); [| specialize (IHt2 context no_free_vars_2 cant_bind cant_bind_context)]. {
+      intros. apply no_free_vars. apply UsedIn.CaO. exact U. }
+    destruct well_formed_in_acc as [[b2 u2] |] eqn:E2 in IHt2; rewrite E2; invert IHt2. 2: {
+      constructor. intros pair [[NH [NS [NP NL]]] C]. apply (N pair). split. 2: { intro x. specialize (C x) as [C1 C2].
+        split; intros; [apply C1 | apply C2]. { apply BoundIn.TCaO. exact B. } { exact I. } apply UsedIn.CaO. exact U. }
+      repeat split; intro; [apply NH | apply NS | apply NP | apply NL]; apply ARCO; assumption. } destruct (bound_used E2) as [B2 U2].
+    destruct (Map.disjoint_spec (Map.overriding_union cant_bind $ Map.overriding_union b2 u2) $ BoundIn.pattern pattern). 2: {
+      constructor. intros _ [[NH [NS [NP NL]]] C]. apply N. intros x I B. apply BoundIn.pattern_iff in B.
+      apply Map.in_overriding_union in I as [I | I]. { apply (C x). 2: { exact I. } apply BoundIn.TCaP. exact B. }
+      apply Map.in_overriding_union in I as [I | I].
+      * apply NH. apply APCO. exists x. split. { exact B. } apply B2. exact I.
+      * apply NL. apply APCO. exists x. split. { exact B. } apply U2. exact I. }
+    eassert (no_free_vars_1 : _); [| specialize (IHt1 (Map.overriding_union (BoundIn.pattern pattern) context)
+      no_free_vars_1 (Map.overriding_union (BoundIn.pattern pattern) $ Map.overriding_union cant_bind $ Map.overriding_union b2 u2))]. {
+      intros. apply Map.in_overriding_union. destruct (BoundIn.pattern_spec pattern x). { left. apply BoundIn.pattern_iff. exact Y1. }
+      right. apply no_free_vars. apply UsedIn.CaB. { exact N. } exact U. }
+    eassert (cant_bind_context' : _); [| specialize (IHt1 cant_bind_context')]. {
+      intro x. repeat rewrite Map.in_overriding_union. intros [I | I]; [left | right]. { exact I. }
+      left. apply cant_bind_context. exact I. }
+    destruct well_formed_in_acc as [[b1 u1] |] eqn:E1 in IHt1; rewrite E1 in *; invert IHt1. 2: {
+      constructor. intros pair [[NH [NS [NP NL]]] C]. apply (N pair). split. {
+        repeat split; intro NA; [apply NH | apply NS | apply NP | apply NL]; apply ARCB; exact NA. }
+      intro x. specialize (C x) as [C1 C2]. split.
+      * intros B I. apply Map.in_overriding_union in I as [I | I]. {
+          apply NH. apply APCB. { constructor. } exists x. split. { apply BoundIn.pattern_iff. exact I. } exact B. }
+        apply Map.in_overriding_union in I as [I | I]. { eapply C1. 2: { exact I. } apply BoundIn.TCaB. exact B. }
+        apply Map.in_overriding_union in I as [I | I]. { apply B2 in I. eapply NP. apply APCO. exists x. split; assumption. }
+        apply U2 in I. apply NS. apply APCO. exists x. split. { exact I. } exact B.
+      * intro U. apply Map.in_overriding_union. destruct (BoundIn.pattern_spec pattern x). { left. apply BoundIn.pattern_iff. exact Y1. }
+        right. apply C2. apply UsedIn.CaB. { exact N0. } exact U. } destruct (bound_used E1) as [B1 U1].
+    destruct (Map.disjoint_spec b2 b1). 2: {
+      constructor. intros _ [[_ [_ [C _]]] _]. apply C. apply APCO.
+      apply Map.not_disjoint_exists in N as [x [C1 C2]]. exists x. split; [apply B2 | apply B1]; assumption. }
+    destruct (Map.disjoint_spec b2 u1). 2: {
+      constructor. intros _ [[_ [C [_ _]]] _]. apply C. apply APCB. { constructor. }
+      apply Map.not_disjoint_exists in N as [x [C1 C2]]. exists x. split; [apply U1 | apply B2]; assumption. }
+    destruct (Map.disjoint_spec b1 u2); constructor. 2: {
+      intros _ [[_ [C [_ _]]] _]. apply C. apply APCO.
+      apply Map.not_disjoint_exists in N as [x [C1 C2]]. exists x. split; [apply U2 | apply B1]; assumption. }
+    split.
+    + repeat split; intro C; invert C; try solve [apply Y in R as []]; try solve [apply Y1 in R as []];
+      destruct Y as [[NH1 [NS1 [NP1 NL1]]] C1]; destruct Y1 as [[NH2 [NS2 [NP2 NL2]]] C2].
+      * destruct here as [x [Bp B]]. eapply C2. { exact B. } apply Map.in_overriding_union. left. apply BoundIn.pattern_iff. exact Bp.
+      * destruct here as [x [Bp B]]. apply (Y0 x). 2: { apply BoundIn.pattern_iff. exact Bp. }
+        apply Map.in_overriding_union. right. apply Map.in_overriding_union. left. apply B2. exact B.
+      * destruct here as [x [U B]]. eapply (Y3 x); [apply B2 | apply U1]; assumption.
+      * destruct here as [x [U B]]. eapply (Y4 x); [apply B1 | apply U2]; assumption.
+      * destruct here as [x [B1' B2']]. eapply (Y2 x); [apply B2 | apply B1]; assumption.
+      * destruct here as [x [B2' B1']]. eapply (Y2 x); [apply B2 | apply B1]; assumption.
+      * destruct lateral as [].
+      * destruct here as [x [Bp U]]. apply (Y0 x). 2: { apply BoundIn.pattern_iff. exact Bp. }
+        apply Map.in_overriding_union. right. apply Map.in_overriding_union. right. apply U2. exact U.
+    + destruct Y as [[NH1 [NS1 [NP1 NL1]]] C1]. destruct Y1 as [[NH2 [NS2 [NP2 NL2]]] C2]. split; intros.
+      * invert B.
+        -- apply (Y0 x). { apply Map.in_overriding_union. left. exact I. } apply BoundIn.pattern_iff. exact bound_in_pattern.
+        -- apply (C2 x). { assumption. } apply Map.in_overriding_union. right. apply Map.in_overriding_union. left. exact I.
+        -- apply (C1 x). { exact bound_in_another_case. } exact I.
+      * invert U.
+        -- apply no_free_vars_1 in used_in_body. apply Map.in_overriding_union in used_in_body as [I | I]. 2: { exact I. }
+           edestruct not_shadowed as []. apply BoundIn.pattern_iff. exact I.
+        -- apply no_free_vars_2. exact used_in_another_case.
+Qed.
+
+Lemma well_formed_in_spec {t context} (no_free_vars : forall x (U : UsedIn.Term t x), Map.In context x)
+  : Reflect.Bool (WellFormedNegIn context t) $ well_formed_in context t.
+Proof.
+  unfold well_formed_in. destruct (@well_formed_in_acc_spec t context no_free_vars context $ fun _ I => I); constructor.
+  - exact Y.
+  - apply N. exact (pair Map.empty Map.empty).
+Qed.
+
+
+
+Inductive WellFormedInAcc (cant_bind context : Map.set) : Term.term -> Prop :=
   | Ctr ctor
-      : Unshadowed (Term.Ctr ctor)
-  | Var name ownership
-      : Unshadowed (Term.Var name ownership)
+      : WellFormedInAcc cant_bind context $ Term.Ctr ctor
+  | Var {name} (I : Map.In context name) ownership
+      : WellFormedInAcc cant_bind context $ Term.Var name ownership
   | App
-      {function} (Uf : Unshadowed function)
-      {argument} (Ua : Unshadowed argument)
-      (disj_f_a : forall x (Bf : BoundIn.Term function x) (Ua : UsedIn.Term argument x), False)
-      (disj_a_f : forall x (Ba : BoundIn.Term argument x) (Uf : UsedIn.Term function x), False)
-      : Unshadowed (Term.App function argument)
+      {argument cant_bind_in_function} (Uf
+        : forall x, Map.In cant_bind_in_function x <-> (Map.In cant_bind x \/ BoundIn.Term argument x \/ UsedIn.Term argument x))
+      {function cant_bind_in_argument} (Ua
+        : forall x, Map.In cant_bind_in_argument x <-> (Map.In cant_bind x \/ BoundIn.Term function x \/ UsedIn.Term function x))
+      (WFf : WellFormedInAcc cant_bind_in_function context function)
+      (WFa : WellFormedInAcc cant_bind_in_argument context argument)
+      (Db : forall x (Bf : BoundIn.Term function x) (Ba : BoundIn.Term argument x), False)
+      : WellFormedInAcc cant_bind context $ Term.App function argument
   | For
-      {type} (Ut : Unshadowed type)
-      {body} (Ub : Unshadowed body)
-      (disj_t_b : forall x (Bt : BoundIn.Term type x) (Ub : UsedIn.Term body x), False)
-      (disj_b_t : forall x (Bb : BoundIn.Term body x) (Ut : UsedIn.Term type x), False) {variable}
-      (Nt : forall (B : BoundIn.Term type variable), False)
-      (Nb : forall (B : BoundIn.Term body variable), False)
-      : Unshadowed (Term.For variable type body)
+      {variable} (NB : forall (I : Map.In cant_bind variable), False)
+      {type} (NBt : forall (B : BoundIn.Term type variable), False)
+      {body} (NBb : forall (B : BoundIn.Term body variable), False)
+      (NUt : forall (U : UsedIn.Term type variable), False)
+      {cant_bind_in_type} (Ut
+        : forall x, Map.In cant_bind_in_type x <-> (Map.In cant_bind x \/ BoundIn.Term body x \/ UsedIn.Term body x))
+      {tmp_body} (Tb
+        : forall x, Map.In tmp_body x <-> (Map.In cant_bind x \/ BoundIn.Term type x \/ UsedIn.Term type x))
+      {cant_bind_in_body} (Ub : Map.Add variable tt tmp_body cant_bind_in_body)
+      {body_context} (Cb : Map.Add variable tt context body_context)
+      (WFt : WellFormedInAcc cant_bind_in_type context type)
+      (WFb : WellFormedInAcc cant_bind_in_body body_context body)
+      (Db : forall x (Bt : BoundIn.Term type x) (Bb : BoundIn.Term body x), False)
+      : WellFormedInAcc cant_bind context $ Term.For variable type body
   | Cas
-      {body_if_match} (Ub : Unshadowed body_if_match)
-      {other_cases} (Uo : Unshadowed other_cases)
-      (disj_b_o : forall x (Bb : BoundIn.Term body_if_match x) (Uo : UsedIn.Term other_cases x), False)
-      (disj_o_b : forall x (Bo : BoundIn.Term other_cases x) (Ub : UsedIn.Term body_if_match x), False) {pattern}
-      (Nb : forall x (Bp : BoundIn.Pattern pattern x) (Bt : BoundIn.Term body_if_match x), False)
-      (No : forall x (Bp : BoundIn.Pattern pattern x) (Bo : BoundIn.Term other_cases x), False)
-      : Unshadowed (Term.Cas pattern body_if_match other_cases)
+      {pattern} (NB : forall x (Bp : BoundIn.Pattern pattern x) (I : Map.In cant_bind x), False)
+      {other_cases} (NBo : forall x (Bp : BoundIn.Pattern pattern x) (B : BoundIn.Term other_cases x), False)
+      {body_if_match} (NBb : forall x (Bp : BoundIn.Pattern pattern x) (B : BoundIn.Term body_if_match x), False)
+      (NUo : forall x (Bp : BoundIn.Pattern pattern x) (U : UsedIn.Term other_cases x), False)
+      {cant_bind_in_other_cases} (Uo
+        : forall x, Map.In cant_bind_in_other_cases x <-> (
+          Map.In cant_bind x \/ BoundIn.Term body_if_match x \/ UsedIn.Term body_if_match x))
+      {tmp_body_if_match : Map.set} (Tb
+        : forall x, Map.In tmp_body_if_match x <-> (
+          Map.In cant_bind x \/ BoundIn.Term other_cases x \/ UsedIn.Term other_cases x))
+      {cant_bind_in_body_if_match} (Ub
+        : forall x, Map.In cant_bind_in_body_if_match x <-> (
+          BoundIn.Pattern pattern x \/ Map.In tmp_body_if_match x))
+      {body_if_match_context} (Cb
+        : forall x, Map.In body_if_match_context x <-> (
+        BoundIn.Pattern pattern x \/ Map.In context x))
+      (WFo : WellFormedInAcc cant_bind_in_other_cases context other_cases)
+      (WFb : WellFormedInAcc cant_bind_in_body_if_match body_if_match_context body_if_match)
+      (Db : forall x (Bo : BoundIn.Term other_cases x) (Bb : BoundIn.Term body_if_match x), False)
+      : WellFormedInAcc cant_bind context $ Term.Cas pattern body_if_match other_cases
   .
 
-Lemma on_the_tin_acc {acc reserved t reserved' renamed}
-  (E : unshadow_acc acc reserved t = Some (reserved', renamed))
-  (prev : forall x y (Fa : Map.Find acc x y), Map.In reserved y)
-  : Unshadowed renamed.
+Definition WellFormedIn context := WellFormedInAcc context context.
+Arguments WellFormedIn context t/.
+
+Lemma eq_acc {r1 c1 t1} (WF : WellFormedInAcc r1 c1 t1)
+  {r2} (Er : Map.Eq r1 r2) {c2} (Ec : Map.Eq c1 c2) {t2} (Et : t1 = t2)
+  : WellFormedInAcc r2 c2 t2.
 Proof.
-  generalize dependent renamed. generalize dependent reserved'.
-  generalize dependent reserved. generalize dependent acc. induction t; intros; cbn in *.
-  - invert E. constructor.
-  - destruct (Map.find_spec acc name); cbn in E; invert E; constructor.
-  - destruct unshadow_acc as [[reserved1 renamed1] |] eqn:E1 in E. 2: { discriminate E. }
-    destruct unshadow_acc as [[reserved2 renamed2] |] eqn:E2 in E; invert E.
-    specialize (IHt1 _ _ prev _ _ E1). eassert (prev' : _); [| specialize (IHt2 _ _ prev' _ _ E2)]. {
-      intros. eapply bindings. { exact E1. } { exact prev. } right. eapply prev. exact Fa. }
-    constructor; try assumption; intros.
-    + eapply disjoint_bound; try exact Bf; try eassumption.
-      assert (I : Map.In reserved1 x). { eapply bindings. { exact E1. } { exact prev. } left. exact Bf. }
-      destruct (disjoint_used E2 prev' I Ua) as [z F]. eapply prev. exact F.
-    + eapply disjoint_bound; try exact Ba; try eassumption.
-      eapply used_reserved. 3: { exact Uf. } { eassumption. } exact prev.
-  - destruct unshadow_acc as [[reserved1 renamed1] |] eqn:E1 in E. 2: { discriminate E. }
-    destruct unshadow_acc as [[reserved2 renamed2] |] eqn:E2 in E; invert E.
-    specialize (IHt1 _ _ prev _ _ E1). eassert (prev' : _); [| specialize (IHt2 _ _ prev' _ _ E2)]. {
-      intros. apply Map.in_overriding_add. apply Map.find_overriding_add in Fa as [[-> ->] | [Na Fa]]. { left. reflexivity. }
-      right. eapply bindings. { exact E1. } { exact prev. } right. eapply prev. exact Fa. }
-    constructor; try assumption; intros.
-    + eapply disjoint_bound; try exact Bt; try eassumption.
-      assert (I : Map.In reserved1 x). { eapply bindings. { exact E1. } { exact prev. } left. exact Bt. }
-      eassert (I' : _); [| destruct (disjoint_used E2 prev' I' Ub) as [z F]]. { apply Map.in_overriding_add. right. exact I. }
-      apply Map.find_overriding_add in F as [[-> ->] | [N F]]. { apply NewNames.not_in_new_name in I as []. } eapply prev. exact F.
-    + eapply disjoint_bound; try exact Ba; try eassumption. apply Map.in_overriding_add.
-      destruct (String.eqb_spec x (NewNames.new_name reserved1 variable)); [left | right]. { assumption. }
-      eapply used_reserved. 3: { exact Ut. } { eassumption. } exact prev.
-    + eapply NewNames.not_in_new_name. eapply bindings. 3: { left. exact B. } { eassumption. } exact prev.
-    + eapply disjoint_bound. { exact E2. } { exact prev'. } 2: { exact B. } apply Map.in_overriding_add. left. reflexivity.
-  - destruct unshadow_acc as [[reserved2 renamed2] |] eqn:E2 in E. 2: { discriminate E. }
-    destruct (@Rename.pattern_spec (Map.fold (fun k _ acc' => Map.overriding_add k (NewNames.new_name
-      (Map.overriding_union reserved2 (Map.fold (fun _ v acc'' => Map.overriding_add v tt acc'') Map.empty acc'))
-      k) acc') Map.empty (BoundIn.pattern pattern)) (NewNames.one_to_one_generate _ _) pattern). 2: { discriminate E. }
-    destruct unshadow_acc as [[reserved1 renamed1] |] eqn:E1 in E; invert E.
-    specialize (IHt2 _ _ prev _ _ E2). eassert (prev' : _); [| specialize (IHt1 _ _ prev' _ _ E1)]. {
-      intros k v F. apply Map.in_overriding_union. rewrite Map.in_range.
-      apply Map.bulk_overwrite_bulk_overwrite in F as [F | [N F]]. { left. eexists. exact F. }
-      right. eapply bindings. { exact E2. } { exact prev. } right. eapply prev. exact F. }
-    constructor; try assumption; intros.
-    + eapply disjoint_bound; try exact Bb; try eassumption. apply Map.in_overriding_union. rewrite Map.in_range.
-      right. eapply used_reserved. { eassumption. } { exact prev. } exact Uo.
-    + eapply disjoint_bound; try exact Bo; try eassumption.
-      assert (I : Map.In reserved2 x0). { eapply bindings. { exact E2. } { exact prev. } left. exact Bo. }
-      eassert (I' : _); [| destruct (disjoint_used E1 prev' I' Ub) as [z F]]. { apply Map.in_overriding_union. right. exact I. }
-      apply Map.bulk_overwrite_bulk_overwrite in F as [F | [N F]]. 2: { eapply prev. exact F. }
-      eassert (IR : Map.InRange _ _). { eexists. exact F. } eapply NewNames.not_in_generate in IR as []. exact I.
-    + apply (Rename.bound_in_pattern Y) in Bp as [z [B F]].
-      eapply disjoint_bound. { exact E1. } { exact prev'. } 2: { exact Bt. }
-      apply Map.in_overriding_union. left. apply Map.in_range. eexists. exact F.
-    + apply (Rename.bound_in_pattern Y) in Bp as [z [B F]].
-      eapply NewNames.not_in_generate. 2: { eexists. exact F. }
-      eapply bindings. 3: { left. exact Bo. } { exact E2. } exact prev.
+  subst. rename t2 into t. generalize dependent c2. generalize dependent r2. induction WF; intros.
+  - constructor.
+  - constructor. eapply Map.in_eq. 2: { exact I. } apply Map.eq_sym. exact Ec.
+  - econstructor; try exact Db; try apply IHWF1; try apply IHWF2; try apply Map.eq_refl; try exact Ec.
+    + intro x. rewrite Uf. split; (intros [I | [B | U]]; [left | right; left; exact B | right; right; exact U]);
+      (eapply Map.in_eq; [| exact I]). 2: { exact Er. } apply Map.eq_sym. exact Er.
+    + intro x. rewrite Ua. split; (intros [I | [B | U]]; [left | right; left; exact B | right; right; exact U]);
+      (eapply Map.in_eq; [| exact I]). 2: { exact Er. } apply Map.eq_sym. exact Er.
+  - econstructor.
+    + intro I. apply NB. eapply Map.in_eq. 2: { exact I. } apply Er.
+    + exact NBt.
+    + exact NBb.
+    + exact NUt.
+    + intro x. rewrite Ut. erewrite (Map.in_eq Er). reflexivity.
+    + intro x. rewrite Tb. erewrite (Map.in_eq Er). reflexivity.
+    + exact Ub.
+    + eapply Map.add_eq. { exact Cb. } { reflexivity. } { reflexivity. } { exact Ec. } apply Map.eq_refl.
+    + apply IHWF1. { apply Map.eq_refl. } exact Ec.
+    + apply IHWF2. { apply Map.eq_refl. } apply Map.eq_refl.
+    + intros. apply (Db x). { exact Bt. } exact Bb.
+  - econstructor.
+    + intros x B I. apply (NB x). { exact B. } eapply Map.in_eq. 2: { exact I. } apply Er.
+    + exact NBo.
+    + exact NBb.
+    + exact NUo.
+    + intro x. rewrite Uo. erewrite (Map.in_eq Er). reflexivity.
+    + intro x. rewrite Tb. erewrite (Map.in_eq Er). reflexivity.
+    + intro x. rewrite Ub. reflexivity.
+    + intro x. rewrite Cb. rewrite (Map.in_eq Ec). reflexivity.
+    + apply IHWF1. { apply Map.eq_refl. } exact Ec.
+    + apply IHWF2. { apply Map.eq_refl. } apply Map.eq_refl.
+    + intros. apply (Db x). { exact Bo. } exact Bb.
 Qed.
 
-Lemma on_the_tin_reserve {reserved t renamed} (E : unshadow_reserve reserved t = Some renamed)
-  : Unshadowed renamed.
+Lemma eq {c1 t1} (WF : WellFormedIn c1 t1)
+  {c2} (Ec : Map.Eq c1 c2) {t2} (Et : t1 = t2)
+  : WellFormedIn c2 t2.
+Proof. eapply eq_acc. { exact WF. } { exact Ec. } { exact Ec. } exact Et. Qed.
+
+Lemma neg_acc cant_bind context t
+  : WellFormedInAcc cant_bind context t <-> WellFormedNegInAcc cant_bind context t.
 Proof.
-  cbn in E. destruct unshadow_acc as [[? ?] |] eqn:Ea; invert E. eapply on_the_tin_acc in Ea. { exact Ea. }
-  intros k v F. apply Map.in_overriding_union. right. rewrite Map.in_range. eexists. exact F.
+  split; intro WF.
+  - induction WF; cbn in *.
+    + split. { repeat split; intro C; invert C. } split; intros. { invert B. } invert U.
+    + split. { repeat split; intro C; invert C. } split; intros. { invert B. } invert U. exact I.
+    + split.
+      * repeat split; intro C; invert C; try solve [destruct here as [_ [[] _]]];
+        try solve [apply IHWF1 in R as []]; try solve [apply IHWF2 in R as []].
+        -- destruct here as [x [U B]]. eapply IHWF2. { exact B. } apply Ua. right. right. exact U.
+        -- destruct here as [x [U B]]. eapply IHWF1. { exact B. } apply Uf. right. right. exact U.
+        -- destruct here as [x [Bf Ba]]. apply (Db x). { exact Bf. } exact Ba.
+        -- destruct here as [x [Ba Bf]]. apply (Db x). { exact Bf. } exact Ba.
+      * split; intros.
+        -- invert B; [eapply IHWF1 | eapply IHWF2]; try eassumption; [apply Uf | apply Ua]; left; exact I.
+        -- invert U; [apply IHWF1 | apply IHWF2]; assumption.
+    + destruct IHWF1 as [[Ht [St [Pt Lt]]] IHt]; destruct IHWF2 as [[Hb [Sb [Pb Lb]]] IHb]. split.
+      * repeat split; intro C; invert C.
+        -- destruct here as [x [<- B]]. apply NBt in B as [].
+        -- destruct here as [x [<- B]]. apply NBb in B as [].
+        -- apply Ht in R as [].
+        -- apply Hb in R as [].
+        -- destruct here as [x [U B]]. eapply IHb in B as [].
+           do 2 eapply or_intror in U. apply Tb in U as [[] U]. exists tt. apply Ub. right. exact U.
+        -- destruct here as [x [U B]]. eapply IHt in B as []. apply Ut. right. right. exact U.
+        -- apply St in R as [].
+        -- apply Sb in R as [].
+        -- destruct here as [x [Bt Bb]]. apply (Db x). { exact Bt. } exact Bb.
+        -- destruct here as [x [Bb Bt]]. apply (Db x). { exact Bt. } exact Bb.
+        -- apply Pt in R as [].
+        -- apply Pb in R as [].
+        -- destruct here as [x [<- U]]. apply NUt in U as [].
+        -- destruct lateral as [].
+        -- apply Lt in R as [].
+        -- apply Lb in R as [].
+      * split; intros.
+        -- invert B; [apply NB in I as [] | |]. { eapply IHt. { exact bound_in_type. } apply Ut. left. exact I. }
+           eapply IHb. { exact bound_in_body. } eapply or_introl in I. apply Tb in I as [[] F]. exists tt. apply Ub. right. exact F.
+        -- invert U. { apply IHt. exact used_in_type. } eapply IHb in used_in_body as [[] U].
+           apply Cb in U as [[E _] | U]. { apply not_shadowed in E as []. } exists tt. exact U.
+    + destruct IHWF1 as [[Hb [Sb [Pb Lb]]] IHo]. destruct IHWF2 as [[Ho [So [Po Lo]]] IHb]. split.
+      * repeat split; intro C; invert C.
+        -- destruct here as [x [Bp B]]. apply NBb in B as []. exact Bp.
+        -- destruct here as [x [Bp B]]. apply NBo in B as []. exact Bp.
+        -- apply Ho in R as [].
+        -- apply Hb in R as [].
+        -- destruct here as [x [U B]]. eapply IHo in B as []. apply Uo. right. right. exact U.
+        -- destruct here as [x [U B]]. eapply IHb in B as []. apply Ub. right. apply Tb. right. right. exact U.
+        -- apply So in R as [].
+        -- apply Sb in R as [].
+        -- destruct here as [x [Bo Bb]]. apply (Db x). { exact Bb. } exact Bo.
+        -- destruct here as [x [Bb Bo]]. apply (Db x). { exact Bb. } exact Bo.
+        -- apply Po in R as [].
+        -- apply Pb in R as [].
+        -- destruct lateral as [].
+        -- destruct here as [x [Bp U]]. apply NUo in U as []. exact Bp.
+        -- apply Lo in R as [].
+        -- apply Lb in R as [].
+      * split; intros.
+        -- invert B; [apply NB in I as []; exact bound_in_pattern | |].
+           ++ eapply IHb. { exact bound_in_body. } apply Ub. right. eapply or_introl in I. apply Tb in I. exact I.
+           ++ eapply IHo. { exact bound_in_another_case. } apply Uo. left. exact I.
+        -- invert U. 2: { apply IHo. exact used_in_another_case. } eapply IHb in used_in_body as I.
+           apply Cb in I as [B | I]. { apply not_shadowed in B as []. } exact I.
+  - generalize dependent context. generalize dependent cant_bind. induction t; intros; cbn in *.
+    + constructor.
+    + constructor. apply WF. constructor.
+    + destruct WF as [[NH [NS [NP NL]]] WF]. econstructor.
+      * split.
+        -- intro I. apply Map.in_overriding_union in I as [I | I]; [left | right]. { exact I. }
+           apply Map.in_overriding_union in I as [I | I]; [left | right];
+           [apply BoundIn.term_iff | apply UsedIn.term_iff]; exact I.
+        -- intro IBU. repeat rewrite Map.in_overriding_union. destruct IBU as [I | [B | U]]; [left; exact I | |]; right;
+           [left | right]; [apply BoundIn.term_iff | apply UsedIn.term_iff]; assumption.
+      * split.
+        -- intro I. apply Map.in_overriding_union in I as [I | I]; [left | right]. { exact I. }
+           apply Map.in_overriding_union in I as [I | I]; [left | right];
+           [apply BoundIn.term_iff | apply UsedIn.term_iff]; exact I.
+        -- intro IBU. repeat rewrite Map.in_overriding_union. destruct IBU as [I | [B | U]]; [left; exact I | |]; right;
+           [left | right]; [apply BoundIn.term_iff | apply UsedIn.term_iff]; assumption.
+      * apply IHt1. split. { repeat split; intro C; [apply NH | apply NS | apply NP | apply NL]; apply ARAF; exact C. }
+        split. 2: { intro U. apply WF. apply UsedIn.ApF. exact U. }
+        intros. apply Map.in_overriding_union in I as [I | I]. { eapply WF. 2: { exact I. } apply BoundIn.TApF. exact B. }
+        apply Map.in_overriding_union in I as [I | I]; [apply BoundIn.term_iff in I | apply UsedIn.term_iff in I].
+        -- apply NP. apply APAF. { constructor. } exists x. split. { exact B. } exact I.
+        -- apply NS. apply APAA. { constructor. } exists x. split. { exact I. } exact B.
+      * apply IHt2. split. { repeat split; intro C; [apply NH | apply NS | apply NP | apply NL]; apply ARAA; exact C. }
+        split. 2: { intro U. apply WF. apply UsedIn.ApA. exact U. }
+        intros. apply Map.in_overriding_union in I as [I | I]. { eapply WF. 2: { exact I. } apply BoundIn.TApA. exact B. }
+        apply Map.in_overriding_union in I as [I | I]; [apply BoundIn.term_iff in I | apply UsedIn.term_iff in I].
+        -- apply NP. apply APAA. { constructor. } exists x. split. { exact B. } exact I.
+        -- apply NS. apply APAF. { constructor. } exists x. split. { exact I. } exact B.
+      * intros. apply NP. apply APAF. { constructor. } exists x. split. { exact Bf. } exact Ba.
+    + destruct WF as [[NH [NS [NP NL]]] WF]. econstructor.
+      * apply WF. apply BoundIn.TFoV.
+      * intro B. apply NH. apply APFT. exists variable. split. { reflexivity. } exact B.
+      * intro B. apply NH. apply APFB. { constructor. } exists variable. split. { reflexivity. } exact B.
+      * intro U. apply NL. apply APFT. exists variable. split. { reflexivity. } exact U.
+      * split.
+        -- intro I. apply Map.in_overriding_union in I as [I | I]; [left | right]. { exact I. }
+           apply Map.in_overriding_union in I as [I | I]; [left | right];
+           [apply BoundIn.term_iff | apply UsedIn.term_iff]; exact I.
+        -- intro IBU. repeat rewrite Map.in_overriding_union. destruct IBU as [I | [B | U]]; [left; exact I | |]; right;
+           [left | right]; [apply BoundIn.term_iff | apply UsedIn.term_iff]; assumption.
+      * split.
+        -- intro I. apply Map.in_overriding_union in I as [I | I]; [left | right]. { exact I. }
+           apply Map.in_overriding_union in I as [I | I]; [left | right];
+           [apply BoundIn.term_iff | apply UsedIn.term_iff]; exact I.
+        -- intro IBU. repeat rewrite Map.in_overriding_union. destruct IBU as [I | [B | U]]; [left; exact I | |]; right;
+           [left | right]; [apply BoundIn.term_iff | apply UsedIn.term_iff]; assumption.
+      * apply Map.add_set.
+      * apply Map.add_set.
+      * apply IHt1. split. { repeat split; intro C; [apply NH | apply NS | apply NP | apply NL]; apply ARFT; exact C. }
+        split. 2: { intro U. apply WF. apply UsedIn.FoT. exact U. }
+        intros. apply Map.in_overriding_union in I as [I | I]. { eapply WF. 2: { exact I. } apply BoundIn.TFoT. exact B. }
+        apply Map.in_overriding_union in I as [I | I]; [apply BoundIn.term_iff in I | apply UsedIn.term_iff in I].
+        -- apply NP. apply APFT. exists x. split. { exact B. } exact I.
+        -- apply NS. apply APFB. { constructor. } exists x. split. { exact I. } exact B.
+      * apply IHt2. split. { repeat split; intro C; [apply NH | apply NS | apply NP | apply NL]; apply ARFB; exact C. }
+        split. 2: { intro U. apply Map.in_overriding_add. destruct (String.eqb_spec x variable); [left | right]. { exact e. }
+          apply WF. apply UsedIn.FoB. 2: { exact U. } exact n. }
+        intros. apply Map.in_overriding_add in I as [-> | I]. {
+          apply NH. apply APFB. { constructor. } exists variable. split. { reflexivity. } exact B. }
+        apply Map.in_overriding_union in I as [I | I]. { apply (WF x). 2: { exact I. } apply BoundIn.TFoB. exact B. }
+        apply Map.in_overriding_union in I as [I | I]; [apply BoundIn.term_iff in I | apply UsedIn.term_iff in I].
+        -- apply NP. apply APFT. exists x. split. { exact I. } exact B.
+        -- apply NS. apply APFT. exists x. split. { exact I. } exact B.
+      * intros. apply NP. apply APFT. exists x. split. { exact Bt. } exact Bb.
+    + destruct WF as [[NH [NS [NP NL]]] WF]. econstructor.
+      * intros x B. apply WF. apply BoundIn.TCaP. exact B.
+      * intros x Bp B. apply NH. apply APCO. exists x. split. { exact Bp. } exact B.
+      * intros x Bp B. apply NH. apply APCB. { constructor. } exists x. split. { exact Bp. } exact B.
+      * intros x Bp U. apply NL. apply APCO. exists x. split. { exact Bp. } exact U.
+      * split.
+        -- intro I. apply Map.in_overriding_union in I as [I | I]; [left | right]. { exact I. }
+           apply Map.in_overriding_union in I as [I | I]; [left | right];
+           [apply BoundIn.term_iff | apply UsedIn.term_iff]; exact I.
+        -- intro IBU. repeat rewrite Map.in_overriding_union. destruct IBU as [I | [B | U]]; [left; exact I | |]; right;
+           [left | right]; [apply BoundIn.term_iff | apply UsedIn.term_iff]; assumption.
+      * split.
+        -- intro I. apply Map.in_overriding_union in I as [I | I]; [left | right]. { exact I. }
+           apply Map.in_overriding_union in I as [I | I]; [left | right];
+           [apply BoundIn.term_iff | apply UsedIn.term_iff]; exact I.
+        -- intro IBU. repeat rewrite Map.in_overriding_union. destruct IBU as [I | [B | U]]; [left; exact I | |]; right;
+           [left | right]; [apply BoundIn.term_iff | apply UsedIn.term_iff]; assumption.
+      * intro x. assert (B := BoundIn.pattern_iff). cbn in B. rewrite <- B. apply Map.in_overriding_union.
+      * intro x. assert (B := BoundIn.pattern_iff). cbn in B. rewrite <- B. apply Map.in_overriding_union.
+      * apply IHt2. split. { repeat split; intro C; [apply NH | apply NS | apply NP | apply NL]; apply ARCO; exact C. }
+        split. 2: { intro U. apply WF. apply UsedIn.CaO. exact U. }
+        intros. apply Map.in_overriding_union in I as [I | I]. { apply (WF x). { apply BoundIn.TCaO. exact B. } exact I. }
+        apply Map.in_overriding_union in I as [I | I]; [apply BoundIn.term_iff in I | apply UsedIn.term_iff in I].
+        -- apply NP. apply APCB. { constructor. } exists x. split. { exact I. } exact B.
+        -- apply NS. apply APCB. { constructor. } exists x. split. { exact I. } exact B.
+      * apply IHt1. split. { repeat split; intro C; [apply NH | apply NS | apply NP | apply NL]; apply ARCB; exact C. }
+        split; intros. 2: { apply Map.in_overriding_union.
+          destruct (BoundIn.pattern_spec pattern x); [left | right]. { apply BoundIn.pattern_iff. exact Y. }
+          apply WF. apply UsedIn.CaB. { exact N. } exact U. }
+        apply Map.in_overriding_union in I as [I | I]. {
+          apply BoundIn.pattern_iff in I. apply NH. apply APCB. { constructor. } exists x. split. { exact I. } exact B. }
+        apply Map.in_overriding_union in I as [I | I]. { apply (WF x). 2: { exact I. } apply BoundIn.TCaB. exact B. }
+        apply Map.in_overriding_union in I as [I | I]; [apply BoundIn.term_iff in I | apply UsedIn.term_iff in I].
+        -- apply NP. apply APCB. { constructor. } exists x. split. { exact B. } exact I.
+        -- apply NS. apply APCO. exists x. split. { exact I. } exact B.
+      * intros. apply NP. apply APCO. exists x. split. { exact Bo. } exact Bb.
 Qed.
 
-Lemma on_the_tin {t renamed} (E : unshadow t = Some renamed)
-  : Unshadowed renamed.
-Proof. apply on_the_tin_reserve in E. exact E. Qed.
+Lemma neg context t
+  : WellFormedIn context t <-> WellFormedNegIn context t.
+Proof. apply neg_acc. Qed.
+
+Lemma context_superset {cant_bind lil t} (WF : WellFormedInAcc cant_bind lil t)
+  {big} (subset : Map.Subset lil big)
+  : WellFormedInAcc cant_bind big t.
+Proof.
+  generalize dependent subset. generalize dependent big. induction WF; intros; cbn in *.
+  - constructor.
+  - constructor. destruct I as [[] F]. exists tt. apply subset. exact F.
+  - econstructor. { exact Uf. } { exact Ua. } { apply IHWF1. exact subset. } { apply IHWF2. exact subset. } exact Db.
+  - econstructor. { exact NB. } { exact NBt. } { exact NBb. } { exact NUt. } { exact Ut. } { exact Tb. } { exact Ub. }
+    { apply Map.add_set. } { apply IHWF1. exact subset. } 2: { exact Db. } apply IHWF2. intros. apply Map.add_set.
+    apply Cb in F as [[-> ->] | F]; [left | right]. { split; reflexivity. } apply subset. exact F.
+  - econstructor. { exact NB. } { exact NBo. } { exact NBb. } { exact NUo. } { exact Uo. } { exact Tb. } { exact Ub. }
+    { intro x. rewrite <- (BoundIn.pattern_iff pattern x). apply Map.in_overriding_union. } { apply IHWF1. exact subset. }
+    2: { exact Db. } apply IHWF2. intros k [] F. apply Map.union_set. eassert (I : Map.In _ _). { exists tt. exact F. }
+    apply Cb in I as [I | I]; [left | right]. { apply BoundIn.pattern_iff in I as [[] F']. exact F'. }
+    destruct I as [[] F']. apply subset. exact F'.
+Qed.
+
+Lemma cant_bind_subset {big context t} (WF : WellFormedInAcc big context t)
+  {lil} (subset : Map.Subset lil big)
+  : WellFormedInAcc lil context t.
+Proof.
+  generalize dependent subset. generalize dependent lil. induction WF; intros; cbn in *.
+  - constructor.
+  - constructor. exact I.
+  - econstructor; intros.
+    + rewrite <- (BoundIn.term_iff argument x). rewrite <- (UsedIn.term_iff argument x).
+      repeat rewrite <- Map.in_overriding_union. reflexivity.
+    + rewrite <- (BoundIn.term_iff function x). rewrite <- (UsedIn.term_iff function x).
+      repeat rewrite <- Map.in_overriding_union. reflexivity.
+    + apply IHWF1. intros x [] F. eassert (I : @Map.In unit _ _). 2: { destruct I as [[] F']. exact F'. }
+      apply Uf. apply Map.union_set in F as [F | F]; [left | right]. { exists tt. eapply subset. exact F. }
+      apply Map.union_set in F as [F | F]; [left | right]. { apply BoundIn.term_iff. exists tt. exact F. }
+      apply UsedIn.term_iff. exists tt. exact F.
+    + apply IHWF2. intros x [] F. eassert (I : @Map.In unit _ _). 2: { destruct I as [[] F']. exact F'. }
+      apply Ua. apply Map.union_set in F as [F | F]; [left | right]. { exists tt. eapply subset. exact F. }
+      apply Map.union_set in F as [F | F]; [left | right]. { apply BoundIn.term_iff. exists tt. exact F. }
+      apply UsedIn.term_iff. exists tt. exact F.
+    + apply (Db x). { exact Bf. } exact Ba.
+  - econstructor; intros.
+    + destruct I as [[] F]. apply NB. exists tt. apply subset. exact F.
+    + apply NBt in B as [].
+    + apply NBb in B as [].
+    + apply NUt in U as [].
+    + rewrite <- (BoundIn.term_iff body x). rewrite <- (UsedIn.term_iff body x).
+      repeat rewrite <- Map.in_overriding_union. reflexivity.
+    + rewrite <- (BoundIn.term_iff type x). rewrite <- (UsedIn.term_iff type x).
+      repeat rewrite <- Map.in_overriding_union. reflexivity.
+    + apply Map.add_set.
+    + apply Map.add_set.
+    + apply IHWF1. intros x [] F. eassert (I : @Map.In unit _ _). 2: { destruct I as [[] F']. exact F'. }
+      apply Ut. apply Map.union_set in F as [F | F]; [left | right]. { exists tt. eapply subset. exact F. }
+      apply Map.union_set in F as [F | F]; [left | right]. { apply BoundIn.term_iff. exists tt. exact F. }
+      apply UsedIn.term_iff. exists tt. exact F.
+    + eapply context_superset; [apply IHWF2 |]. 2: {
+        intros x [] F. apply Map.add_set. apply Cb in F as [[-> _] | F]; [left | right]. { split; reflexivity. } exact F. }
+      intros x [] F. apply Ub. apply Map.add_set in F as [E | F]; [left | right]. { exact E. }
+      eassert (I : @Map.In unit _ _). 2: { destruct I as [[] F']. exact F'. } apply Tb.
+      apply Map.union_set in F as [F | F]; [left | right]. { exists tt. apply subset. exact F. }
+      apply Map.union_set in F as [F | F]; [left | right]. { apply BoundIn.term_iff. exists tt. exact F. }
+      apply UsedIn.term_iff. exists tt. exact F.
+    + apply (Db x). { exact Bt. } exact Bb.
+  - econstructor; intros.
+    + destruct I as [[] F]. apply (NB x). { exact Bp. } exists tt. apply subset. exact F.
+    + apply NBo in B as []. exact Bp.
+    + apply NBb in B as []. exact Bp.
+    + apply NUo in U as []. exact Bp.
+    + rewrite <- (BoundIn.term_iff body_if_match x). rewrite <- (UsedIn.term_iff body_if_match x).
+      repeat rewrite <- Map.in_overriding_union. reflexivity.
+    + rewrite <- (BoundIn.term_iff other_cases x). rewrite <- (UsedIn.term_iff other_cases x).
+      repeat rewrite <- Map.in_overriding_union. reflexivity.
+    + rewrite <- (BoundIn.pattern_iff pattern x). apply Map.in_overriding_union.
+    + rewrite <- (BoundIn.pattern_iff pattern x). apply Map.in_overriding_union.
+    + apply IHWF1. intros x [] F. eassert (I : @Map.In unit _ _). 2: { destruct I as [[] F']. exact F'. }
+      apply Uo. apply Map.union_set in F as [F | F]; [left | right]. { exists tt. eapply subset. exact F. }
+      apply Map.union_set in F as [F | F]; [left | right]. { apply BoundIn.term_iff. exists tt. exact F. }
+      apply UsedIn.term_iff. exists tt. exact F.
+    + eapply context_superset; [apply IHWF2 |]. 2: {
+        intros x [] F. apply Map.union_set. eassert (I : Map.In _ _). { exists tt. exact F. }
+        apply Cb in I as [I | I]; [left | right]. { apply BoundIn.pattern_iff in I as [[] F']. exact F'. }
+        destruct I as [[] F']. exact F'. }
+      intros x [] F. eassert (I : @Map.In unit _ _). 2: { destruct I as [[] F']. exact F'. } apply Ub.
+      apply Map.union_set in F as [F | F]; [left | right]. { apply BoundIn.pattern_iff. exists tt. exact F. }
+      apply Tb. apply Map.union_set in F as [F | F]; [left | right]. { exists tt. apply subset. exact F. }
+      apply Map.union_set in F as [F | F]; [left | right]. { apply BoundIn.term_iff. exists tt. exact F. }
+      apply UsedIn.term_iff. exists tt. exact F.
+    + apply (Db x). { exact Bo. } exact Bb.
+Qed.
+
+Lemma cant_bind_union {lil context t} (WF : WellFormedInAcc lil context t)
+  {marginal big} (union : Map.Union lil marginal big) (NB : forall x (B : BoundIn.Term t x) (I : Map.In marginal x), False)
+  : WellFormedInAcc big context t.
+Proof.
+  generalize dependent big. generalize dependent marginal. induction WF; intros; cbn in *.
+  - constructor.
+  - constructor. exact I.
+  - econstructor; intros.
+    + rewrite <- (BoundIn.term_iff argument x). rewrite <- (UsedIn.term_iff argument x).
+      repeat rewrite <- Map.in_overriding_union. reflexivity.
+    + rewrite <- (BoundIn.term_iff function x). rewrite <- (UsedIn.term_iff function x).
+      repeat rewrite <- Map.in_overriding_union. reflexivity.
+    + eapply IHWF1. { intros. apply (NB x). { apply BoundIn.TApF. exact B. } exact I. } intros x []. split.
+      * intro F. apply Map.union_set in F as [F | F].
+        -- apply union in F as [F | F]. 2: { right. exact F. }
+           left. eassert (I : @Map.In unit _ _). 2: { destruct I as [[] F']. exact F'. }
+           apply Uf. left. exists tt. exact F.
+        -- left. eassert (I : @Map.In unit _ _). 2: { destruct I as [[] F']. exact F'. }
+           apply Uf. right. apply Map.union_set in F as [F | F]; [left | right];
+           [apply BoundIn.term_iff | apply UsedIn.term_iff]; exists tt; assumption.
+      * intro FF. apply Map.union_set. rewrite union. destruct FF as [F | F]. 2: { left. right. exact F. }
+        eassert (I : Map.In _ _). { exists tt. exact F. } apply Uf in I as [[[] F'] | I]. { left. left. exact F'. }
+        right. apply Map.union_set. destruct I as [B | U]; [left | right];
+        [apply BoundIn.term_iff in B as [[] F'] | apply UsedIn.term_iff in U as [[] F']]; exact F'.
+    + eapply IHWF2. { intros. apply (NB x). { apply BoundIn.TApA. exact B. } exact I. } intros x []. split.
+      * intro F. apply Map.union_set in F as [F | F].
+        -- apply union in F as [F | F]. 2: { right. exact F. }
+           left. eassert (I : @Map.In unit _ _). 2: { destruct I as [[] F']. exact F'. }
+           apply Ua. left. exists tt. exact F.
+        -- left. eassert (I : @Map.In unit _ _). 2: { destruct I as [[] F']. exact F'. }
+           apply Ua. right. apply Map.union_set in F as [F | F]; [left | right];
+           [apply BoundIn.term_iff | apply UsedIn.term_iff]; exists tt; assumption.
+      * intro FF. apply Map.union_set. rewrite union. destruct FF as [F | F]. 2: { left. right. exact F. }
+        eassert (I : Map.In _ _). { exists tt. exact F. } apply Ua in I as [[[] F'] | I]. { left. left. exact F'. }
+        right. apply Map.union_set. destruct I as [B | U]; [left | right];
+        [apply BoundIn.term_iff in B as [[] F'] | apply UsedIn.term_iff in U as [[] F']]; exact F'.
+    + apply (Db x). { exact Bf. } exact Ba.
+  - econstructor; intros.
+    + destruct I as [[] F]. apply union in F as [F | F]. { apply NB. exists tt. exact F. }
+      apply (NB0 variable). { apply BoundIn.TFoV. } exists tt. exact F.
+    + apply NBt in B as [].
+    + apply NBb in B as [].
+    + apply NUt in U as [].
+    + rewrite <- (BoundIn.term_iff body x). rewrite <- (UsedIn.term_iff body x).
+      repeat rewrite <- Map.in_overriding_union. reflexivity.
+    + rewrite <- (BoundIn.term_iff type x). rewrite <- (UsedIn.term_iff type x).
+      repeat rewrite <- Map.in_overriding_union. reflexivity.
+    + apply Map.add_set.
+    + apply Map.add_set.
+    + eapply IHWF1. { intros. apply (NB0 x). { apply BoundIn.TFoT. exact B. } exact I. } intros x []. split.
+      * intro F. apply Map.union_set in F as [F | F].
+        -- apply union in F as [F | F]. 2: { right. exact F. }
+           left. eassert (I : @Map.In unit _ _). 2: { destruct I as [[] F']. exact F'. }
+           apply Ut. left. exists tt. exact F.
+        -- left. eassert (I : @Map.In unit _ _). 2: { destruct I as [[] F']. exact F'. }
+           apply Ut. right. apply Map.union_set in F as [F | F]; [left | right];
+           [apply BoundIn.term_iff | apply UsedIn.term_iff]; exists tt; assumption.
+      * intro FF. apply Map.union_set. rewrite union. destruct FF as [F | F]. 2: { left. right. exact F. }
+        eassert (I : Map.In _ _). { exists tt. exact F. } apply Ut in I as [[[] F'] | I]. { left. left. exact F'. }
+        right. apply Map.union_set. destruct I as [B | U]; [left | right];
+        [apply BoundIn.term_iff in B as [[] F'] | apply UsedIn.term_iff in U as [[] F']]; exact F'.
+    + eapply context_superset; [eapply IHWF2 |]. { intros. apply (NB0 x). { apply BoundIn.TFoB. exact B. } exact I. } 2: {
+        intros x [] F. apply Map.add_set. apply Cb. exact F. } intros x []. split.
+      * intro F. apply Map.add_set in F as [[-> _] | F]. { left. apply Ub. left. split; reflexivity. }
+        apply Map.union_set in F as [F | F].
+        -- apply union in F as [F | F]. 2: { right. exact F. }
+           left. eassert (I : @Map.In unit _ _). 2: { destruct I as [[] F']. exact F'. }
+           exists tt. apply Ub. right. eassert (I : @Map.In unit _ _). 2: { destruct I as [[] F']. exact F'. }
+           apply Tb. left. exists tt. exact F.
+        -- left. eassert (I : @Map.In unit _ _). 2: { destruct I as [[] F']. exact F'. }
+           exists tt. apply Ub. right. eassert (I : @Map.In unit _ _). 2: { destruct I as [[] F']. exact F'. }
+           apply Tb. right. apply Map.union_set in F as [F | F]; [left | right];
+           [apply BoundIn.term_iff | apply UsedIn.term_iff]; exists tt; assumption.
+      * intro FF. apply Map.add_set. assert (E := Map.union_set); cbn in E; repeat rewrite E; clear E.
+        rewrite union. destruct FF as [F | F]. 2: { right. left. right. exact F. }
+        apply Ub in F as [E | F]; [left | right]. { exact E. }
+        eassert (I : Map.In _ _). { exists tt. exact F. } apply Tb in I as [[[] F'] | I]. { left. left. exact F'. }
+        right. destruct I as [B | U]; [left | right];
+        [apply BoundIn.term_iff in B as [[] F'] | apply UsedIn.term_iff in U as [[] F']]; exact F'.
+    + apply (Db x). { exact Bt. } exact Bb.
+  - econstructor; intros.
+    + destruct I as [[] F]. apply union in F as [F | F]. { apply (NB x). { exact Bp. } exists tt. exact F. }
+      apply (NB0 x). { apply BoundIn.TCaP. exact Bp. } exists tt. exact F.
+    + apply NBo in B as []. exact Bp.
+    + apply NBb in B as []. exact Bp.
+    + apply NUo in U as []. exact Bp.
+    + rewrite <- (BoundIn.term_iff body_if_match x). rewrite <- (UsedIn.term_iff body_if_match x).
+      repeat rewrite <- Map.in_overriding_union. reflexivity.
+    + rewrite <- (BoundIn.term_iff other_cases x). rewrite <- (UsedIn.term_iff other_cases x).
+      repeat rewrite <- Map.in_overriding_union. reflexivity.
+    + rewrite <- (BoundIn.pattern_iff pattern x). apply Map.in_overriding_union.
+    + rewrite <- (BoundIn.pattern_iff pattern x). apply Map.in_overriding_union.
+    + eapply IHWF1. { intros. apply (NB0 x). { apply BoundIn.TCaO. exact B. } exact I. } intros x []. split.
+      * intro F. apply Map.union_set in F as [F | F].
+        -- apply union in F as [F | F]. 2: { right. exact F. }
+           left. eassert (I : @Map.In unit _ _). 2: { destruct I as [[] F']. exact F'. }
+           apply Uo. left. exists tt. exact F.
+        -- left. eassert (I : @Map.In unit _ _). 2: { destruct I as [[] F']. exact F'. }
+           apply Uo. right. apply Map.union_set in F as [F | F]; [left | right];
+           [apply BoundIn.term_iff | apply UsedIn.term_iff]; exists tt; assumption.
+      * intro FF. apply Map.union_set. rewrite union. destruct FF as [F | F]. 2: { left. right. exact F. }
+        eassert (I : Map.In _ _). { exists tt. exact F. } apply Uo in I as [[[] F'] | I]. { left. left. exact F'. }
+        right. apply Map.union_set. destruct I as [B | U]; [left | right];
+        [apply BoundIn.term_iff in B as [[] F'] | apply UsedIn.term_iff in U as [[] F']]; exact F'.
+    + eapply context_superset; [eapply IHWF2 |]. { intros. apply (NB0 x). { apply BoundIn.TCaB. exact B. } exact I. } 2: {
+        intros x [] F. apply Map.union_set. destruct (Cb x) as [[B | [[] F']] _]; [exists tt; exact F | left | right]. {
+          apply BoundIn.pattern_iff in B as [[] B]. exact B. } exact F'. }
+      intros x []. split.
+      * intro F. apply Map.union_set in F as [F | F]. {
+          left. eassert (I : @Map.In unit _ _). 2: { destruct I as [[] F']. exact F'. }
+          apply Ub. left. apply BoundIn.pattern_iff. exists tt. exact F. }
+        apply Map.union_set in F as [F | F].
+        -- apply union in F as [F | F]. 2: { right. exact F. }
+           left. eassert (I : @Map.In unit _ _). 2: { destruct I as [[] F']. exact F'. }
+           apply Ub. right. apply Tb. left. exists tt. exact F.
+        -- left. eassert (I : @Map.In unit _ _). 2: { destruct I as [[] F']. exact F'. }
+           apply Ub. right. apply Tb. right. apply Map.union_set in F as [F | F]; [left | right];
+           [apply BoundIn.term_iff | apply UsedIn.term_iff]; exists tt; assumption.
+      * intro FF. assert (E := Map.union_set); cbn in E; repeat rewrite E; clear E.
+        rewrite union. destruct FF as [F | F]. 2: { right. left. right. exact F. }
+        eassert (I : Map.In _ _). { exists tt. exact F. }
+        apply Ub in I as [B | I]; [left | right]. { apply BoundIn.pattern_iff in B as [[] F']. exact F'. }
+        apply Tb in I as [[[] F'] | I]; [left | right]. { left. exact F'. }
+        destruct I as [B | U]; [left | right];
+        [apply BoundIn.term_iff in B as [[] F'] | apply UsedIn.term_iff in U as [[] F']]; exact F'.
+    + apply (Db x). { exact Bo. } exact Bb.
+Qed.
 
 
 
-Fixpoint unshadowed_acc t :=
+(* TODO: make sure that bindings are disjoint: i.e., binding the same name implies that two terms are the same *)
+Definition WellFormedContext context : Prop :=
+  forall domain (D : Map.Domain context domain),
+  Map.ForAll (fun _ => Unshadow.WellFormedIn domain) context.
+Arguments WellFormedContext context/.
+
+Definition WellFormedInContext context term : Prop :=
+  WellFormedContext context /\ (* Yes, this `domain` is redundant, but efficiency doesn't matter, and this can be `destruct`ed *)
+  forall domain (D : Map.Domain context domain),
+  Unshadow.WellFormedIn domain term.
+Arguments WellFormedInContext context term/.
+
+
+
+Definition unshadow_context_each k v (acc : option (Map.set * Context.context)) : option (Map.set * Context.context) :=
+  match acc with | None => None | Some (cant_bind, acc) =>
+    match unshadow_reserve_bindings cant_bind v with None => None | Some (bindings, v') =>
+      Some (Map.set_union bindings cant_bind, Map.overriding_add k v' acc)
+    end
+  end.
+Arguments unshadow_context_each k v acc/.
+
+Definition unshadow_context_acc :=
+  Map.fold unshadow_context_each.
+Arguments unshadow_context_acc/ acc context : rename.
+
+Definition unshadow_context (context : Context.context) :=
+  unshadow_context_acc (Some (Map.domain context, Map.empty)) context.
+Arguments unshadow_context context/.
+
+Lemma unfold_right {X Y} (f : X -> Y -> Y) init head tail
+  : List.fold_right f init (head :: tail) = f head $ List.fold_right f init tail.
+Proof. reflexivity. Qed.
+
+Lemma unshadow_context_spec_acc
+  {acc} (Ra : Reflect.Option (fun '(cant_bind', ctx) => Map.ForAll (fun _ => WellFormed.AllPatternsIn) ctx) acc) ctx
+  : Reflect.Option (fun '(cant_bind', ctx') =>
+      Map.ForAll (fun _ => WellFormed.AllPatternsIn) ctx /\
+      Map.ForAll (fun _ => WellFormed.AllPatternsIn) ctx'
+    ) $ unshadow_context_acc acc ctx.
+Proof.
+  unfold unshadow_context_acc. unfold Map.fold. rewrite MapCore.fold_spec. rewrite <- List.fold_left_rev_right.
+  eapply (@Reflect.option_eq _ $ fun '(cant_bind', ctx') => (forall k v (F
+    : SetoidList.InA MapCore.eq_key_elt (k, v) $ List.rev (MapCore.bindings ctx)), _) /\
+      Map.ForAll (fun _ => WellFormed.AllPatternsIn) ctx'). {
+    intros [cant_bind' ctx']. split; intros [H same]; (split; [| exact same]);
+    intros k v F; apply (H k v); [apply -> SetoidList.InA_rev in F |];
+    apply MapCore.bindings_spec1 in F; [| apply SetoidList.InA_rev in F]; exact F. }
+  remember (List.rev (MapCore.bindings ctx)) as b eqn:Eb; clear ctx Eb.
+  generalize dependent acc. induction b as [| [k v] tail IH]; intros. {
+    cbn. destruct acc as [[bindings acc] |]; cbn in *; invert Ra; constructor. {
+      split; intros k v F. { invert F. } eapply Y. exact F. }
+    intros [cant_bind' ctx'] [C C']. apply (N (cant_bind', ctx')). exact C'. }
+  rewrite unfold_right. simpl fst. simpl snd. unfold unshadow_context_each at 1. specialize (IH acc Ra).
+  destruct IH as [[cant_bind' ctx'] [Y Y'] |]. 2: { constructor. intros [cant_bind' ctx'] [C C'].
+    apply (N (cant_bind', ctx')). split. { intros k' v' F'. eapply C. right. exact F'. } exact C'. }
+  destruct (wf_patterns_spec_bindings cant_bind' v) as [[cant_bind'' ctx''] [Y'' Y'''] |]; constructor. 2: {
+    intros [cant_bind'' ctx''] [C C']. eapply (N (cant_bind'', v)). split; eapply C; left; split; reflexivity. }
+  split; intros k' v' F'. { invert F'. { destruct H0. cbn in *. subst. exact Y''. } eapply Y. exact H0. }
+  apply Map.overwrite_if_present_overwrite in F' as [[-> ->] | [N' F']]. { exact Y'''. } eapply Y'. exact F'.
+Qed.
+
+Lemma unshadow_context_spec ctx
+  : Reflect.Option (fun '(cant_bind', ctx') =>
+      Map.ForAll (fun _ => WellFormed.AllPatternsIn) ctx /\
+      Map.ForAll (fun _ => WellFormed.AllPatternsIn) ctx'
+    ) $ unshadow_context ctx.
+Proof.
+  unfold unshadow_context. eassert (A : _); [|
+    destruct (@unshadow_context_spec_acc (Some (Map.domain ctx, Map.empty)) A ctx) as [[cant_bind' ctx'] [Y Y'] |]].
+  - constructor. intros k v C. invert C.
+  - constructor. split. { exact Y. } exact Y'.
+  - constructor. intros [cant_bind' ctx'] [C C']. apply (N (cant_bind', ctx')). split. { exact C. } exact C'.
+Qed.
+
+
+
+(*
+Inductive UnshadowedIn (cant_bind context : Map.set) : Term.term -> Prop :=
+  | Ctr ctor
+      : UnshadowedIn cant_bind context (Term.Ctr ctor)
+  | Var {name} (no_free_variables : Map.In context name) ownership
+      (* TODO: since we enforce that `name` is in `context` (so there are no free variables),
+       * this should be renamed as more of a catch-all well-formed definition than "unshadowed" alone *)
+      : UnshadowedIn cant_bind context (Term.Var name ownership)
+  | App
+      {function} {bound_in_function} (Bf : Map.Reflect (BoundIn.Term function) bound_in_function)
+      {used_in_function} (Uf : Map.Reflect (UsedIn.Term function) used_in_function)
+      {argument} {bound_in_argument} (Ba : Map.Reflect (BoundIn.Term argument) bound_in_argument)
+      {used_in_argument} (Ua : Map.Reflect (UsedIn.Term argument) used_in_argument)
+      {tmp_function} (Tf : Map.Union cant_bind bound_in_argument tmp_function)
+      {cant_bind_in_function} (Cf : Map.Union tmp_function used_in_argument cant_bind_in_function)
+      {tmp_argument} (Tf : Map.Union cant_bind bound_in_function tmp_argument)
+      {cant_bind_in_argument} (Cf : Map.Union tmp_argument used_in_function cant_bind_in_argument)
+      (Uf : UnshadowedIn cant_bind_in_function context function)
+      (Ua : UnshadowedIn cant_bind_in_argument context argument)
+      : UnshadowedIn cant_bind context (Term.App function argument)
+  | For
+      {variable} (N : ~Map.In cant_bind variable)
+      {type} {bound_in_type} (Bt : Map.Reflect (BoundIn.Term type) bound_in_type)
+      {used_in_type} (Ut : Map.Reflect (UsedIn.Term type) used_in_type)
+      {body} {bound_in_body} (Bb : Map.Reflect (BoundIn.Term body) bound_in_body)
+      {used_in_body} (Ub : Map.Reflect (UsedIn.Term body) used_in_body)
+      {tmp_type} (Tt : Map.Union cant_bind bound_in_body tmp_type)
+      {cant_bind_in_type} (Ct : Map.Union tmp_type used_in_body cant_bind_in_type)
+      {tmp_body} (Tb : Map.Union cant_bind bound_in_type tmp_body)
+      {cant_bind_in_body_without_bindings} (Cb : Map.Union tmp_body used_in_type cant_bind_in_body_without_bindings)
+      {cant_bind_in_body} (Cb' : Map.Add variable tt cant_bind_in_body_without_bindings cant_bind_in_body)
+      {context_for_body} (Ab : Map.Add variable tt context context_for_body)
+      (Ut : UnshadowedIn cant_bind_in_type context type)
+      (Ub : UnshadowedIn cant_bind_in_body context_for_body body)
+      : UnshadowedIn cant_bind context (Term.For variable type body)
+  | Cas
+      {pattern bound_in_pattern} (Bp
+        : Map.Reflect (BoundIn.Pattern pattern) bound_in_pattern) (N : Map.Disjoint cant_bind bound_in_pattern)
+      {other_cases} {bound_in_other_cases} (Bo : Map.Reflect (BoundIn.Term other_cases) bound_in_other_cases)
+      {used_in_other_cases} (Uo : Map.Reflect (UsedIn.Term other_cases) used_in_other_cases)
+      {body_if_match} {bound_in_body_if_match} (Bb : Map.Reflect (BoundIn.Term body_if_match) bound_in_body_if_match)
+      {used_in_body_if_match} (Ub : Map.Reflect (UsedIn.Term body_if_match) used_in_body_if_match)
+      {tmp_other_cases} (To : Map.Union cant_bind bound_in_body_if_match tmp_other_cases)
+      {cant_bind_in_other_cases} (Co : Map.Union tmp_other_cases used_in_body_if_match cant_bind_in_other_cases)
+      {tmp_body_if_match} (Tb : Map.Union cant_bind bound_in_body_if_match tmp_body_if_match)
+      {cant_bind_in_body_if_match_without_bindings} (Cb
+        : Map.Union tmp_body_if_match used_in_body_if_match cant_bind_in_body_if_match_without_bindings)
+      {cant_bind_in_body_if_match} (Cb'
+        : Map.Union bound_in_pattern cant_bind_in_body_if_match_without_bindings cant_bind_in_body_if_match)
+      {context_for_body_if_match} (Ab : Map.Union bound_in_pattern context context_for_body_if_match)
+      (Ub : UnshadowedIn cant_bind_in_body_if_match context_for_body_if_match body_if_match)
+      (Uo : UnshadowedIn cant_bind_in_other_cases context other_cases)
+      : UnshadowedIn cant_bind context (Term.Cas pattern body_if_match other_cases)
+  .
+
+Lemma eq {r1 c1 t1} (U : UnshadowedIn r1 c1 t1)
+  {r2} (Er : Map.Eq r1 r2)
+  {c2} (Ec : Map.Eq c1 c2)
+  {t2} (Et : t1 = t2)
+  : UnshadowedIn r2 c2 t2.
+Proof.
+  subst. rename t2 into t. generalize dependent c2. generalize dependent r2. induction U; intros.
+  - constructor.
+  - constructor. eapply Map.in_eq. 2: { exact no_free_variables. } apply Map.eq_sym. exact Ec.
+  - econstructor; try apply IHU1; try apply IHU2; try exact Bf; try exact Ba; try exact Uf; try exact Ua; try apply Map.eq_refl; try eassumption. try apply Map.eq_refl; try eassumption.
+    + eapply Map.union_eq; try exact Cf; try exact Er; try exact Ec; apply Map.eq_refl.
+    + eapply Map.union_eq; try exact Ca; try exact Er; try exact Ec; apply Map.eq_refl.
+  - econstructor; try apply IHU1; try apply IHU2; try apply Map.eq_refl; try eassumption.
+    + intro I. apply N. eapply Map.in_eq. 2: { exact I. } exact Er.
+    + eapply Map.add_eq; try exact Ab; try reflexivity; try eassumption; apply Map.eq_refl.
+    + eapply Map.union_eq; try exact Ct; try exact Er; try exact Ec; apply Map.eq_refl.
+    + eapply Map.union_eq; try exact Cb; try exact Er; try exact Ec; apply Map.eq_refl.
+  - econstructor; try apply IHU1; try apply IHU2; try apply Map.eq_refl; try eassumption.
+    + intros k Ic Ib. eapply N. 2: { exact Ib. } eapply Map.in_eq. 2: { exact Ic. } exact Er.
+    + eapply Map.union_eq; try exact Ab; try exact Ec; apply Map.eq_refl.
+    + eapply Map.union_eq; try exact Cb; try exact Er; try exact Ec; apply Map.eq_refl.
+    + eapply Map.union_eq; try exact Co; try exact Er; try exact Ec; apply Map.eq_refl.
+Qed.
+
+Lemma disj_bound {cant_bind context t} (U : UnshadowedIn cant_bind context t)
+  {x} (I : Map.In cant_bind x) (B : BoundIn.Term t x)
+  : False.
+Proof.
+  destruct I as [[] F]. generalize dependent x. induction U; intros.
+  - invert B.
+  - invert B.
+  - invert B; [eapply IHU1 | eapply IHU2]; try eassumption; [apply Cf | apply Ca]; left; exact F.
+  - invert B; [| eapply IHU1 | eapply IHU2]; try eassumption. { apply N. exists tt. exact F. }
+    + apply Ct. left. exact F.
+    + apply Cb'. right. apply Cb. left. exact F.
+  - invert B; [| eapply IHU1 | eapply IHU2]; try eassumption. { eapply N. { exists tt. exact F. } apply Bp. exact bound_in_pattern0. }
+    + apply Cb'. right. apply Cb. left. exact F.
+    + apply Co. left. exact F.
+Qed.
+
+Lemma used {cant_bind context t} (Ui : UnshadowedIn cant_bind context t) {x} (Ut : UsedIn.Term t x)
+  : Map.In context x.
+Proof.
+  generalize dependent x. induction Ui; intros; cbn in *.
+  - invert Ut.
+  - invert Ut. exact no_free_variables.
+  - invert Ut. { eapply IHUi1. exact used_in_function. } apply IHUi2. exact used_in_argument.
+  - invert Ut. { eapply IHUi1. exact used_in_type. } specialize (IHUi2 _ used_in_body) as [[] IH].
+    apply Ab in IH as [[-> _] | IH]. { contradiction not_shadowed. reflexivity. } exists tt. exact IH.
+  - invert Ut. 2: { eapply IHUi2. exact used_in_another_case. } specialize (IHUi1 _ used_in_body) as [[] IH].
+    apply Ab in IH as [IH | IH]. { contradiction not_shadowed. apply Bp. exists tt. exact IH. } exists tt. exact IH.
+Qed.
+
+Lemma context_superset {cant_bind lil t} (U : UnshadowedIn cant_bind lil t)
+  {big} (S : Map.Subset lil big)
+  : UnshadowedIn cant_bind big t.
+Proof.
+  generalize dependent big. induction U; intros; cbn in *.
+  - constructor.
+  - constructor. destruct no_free_variables as [v F]. exists v. apply S. exact F.
+  - econstructor; try eassumption.
+    + apply IHU1. intros. apply S. exact F.
+    + apply IHU2. intros. apply S. exact F.
+  - econstructor. { exact N. } { exact Bt. } { exact Bb. } { apply Map.add_set. } { exact Ct. } { exact Cb. } { exact Cb'. }
+    + apply IHU1. intros. apply S. exact F.
+    + apply IHU2. intros. apply Map.add_set.
+      apply Ab in F as [[-> ->] | F]; [left | right]. { split; reflexivity. } apply S. exact F.
+  - econstructor. { exact Bp. } { exact N. } { exact Bb. } { exact Bo. }
+    { apply Map.union_set. } { exact Cb. } { exact Cb'. } { exact Co. }
+    + apply IHU1. intros. apply Map.union_set.
+      apply Ab in F as [F | F]; [left | right]. { exact F. } apply S. exact F.
+    + apply IHU2. intros. apply S. exact F.
+Qed.
+
+Lemma cant_bind_union {lil context t} (L : UnshadowedIn lil context t)
+  {marginal} (marginal_not_bound : forall x (I : Map.In marginal x) (B : BoundIn.Term t x), False)
+  {big} (U : Map.Union lil marginal big)
+  : UnshadowedIn big context t.
+Proof.
+  generalize dependent big. generalize dependent marginal. induction L; intros.
+  - constructor.
+  - constructor. exact no_free_variables.
+  - econstructor. { exact Bf. } { exact Ba. } { apply Map.union_set. } { apply Map.union_set. }
+    + eapply IHL1. 2: { intros k []. split.
+      * intro F. apply Map.union_set in F as [F | F]. 2: { left. apply Cf. right. exact F. }
+        apply U in F as [F | F]. 2: { right. exact F. } left. apply Cf. left. exact F.
+      * intros FF. apply Map.union_set. destruct FF as [F | F]. 2: { left. apply U. right. exact F. }
+        apply Cf in F as [F | F]. 2: { right. exact F. } left. apply U. left. exact F. }
+      intros x I B. eapply marginal_not_bound. { exact I. } apply BoundIn.TApF. exact B.
+    + eapply IHL2. 2: { intros k []. split.
+      * intro F. apply Map.union_set in F as [F | F]. 2: { left. apply Ca. right. exact F. }
+        apply U in F as [F | F]. 2: { right. exact F. } left. apply Ca. left. exact F.
+      * intros FF. apply Map.union_set. destruct FF as [F | F]. 2: { left. apply U. right. exact F. }
+        apply Ca in F as [F | F]. 2: { right. exact F. } left. apply U. left. exact F. }
+      intros x I B. eapply marginal_not_bound. { exact I. } apply BoundIn.TApA. exact B.
+  - econstructor; try solve [apply Map.union_set]; try solve [apply Map.add_set]; try eassumption.
+    + intros [[] F]. apply N. apply U in F as [F | F]. { exists tt. exact F. }
+      edestruct marginal_not_bound as []. { exists tt. exact F. } constructor.
+    + eapply IHL1. 2: { intros k []. split.
+      * intro F. apply Map.union_set in F as [F | F]. 2: { left. apply Ct. right. exact F. }
+        apply U in F as [F | F]. 2: { right. exact F. } left. apply Ct. left. exact F.
+      * intros FF. apply Map.union_set. destruct FF as [F | F]. 2: { left. apply U. right. exact F. }
+        apply Ct in F as [F | F]. 2: { right. exact F. } left. apply U. left. exact F. }
+      intros x I B. eapply marginal_not_bound. { exact I. } apply BoundIn.TFoT. exact B.
+    + eapply eq; try reflexivity; try eapply IHL2. 2: { apply Map.union_set. } 3: {
+        eapply Map.add_det; try reflexivity. { exact Ab. } 2: { apply Map.add_set. } apply Map.eq_refl. } 2: { split.
+        * intro F. apply Map.add_set. apply Map.union_set in F as [F | F]. {
+            apply Cb' in F as [E | F]; [left | right]. { exact E. }
+            apply Map.union_set. apply Cb in F as [F | F]; [left | right]. 2: { exact F. } apply U. left. exact F. }
+          right. apply Map.union_set. left. apply U. right. exact F.
+        * intro F. apply Map.union_set. apply Map.add_set in F as [[-> ->] | F]. { left. apply Cb'. left. split; reflexivity. }
+          apply Map.union_set in F as [F | F]. 2: { left. apply Cb'. right. apply Cb. right. exact F. }
+          apply U in F as [F | F]; [left | right]. 2: { exact F. } apply Cb'. right. apply Cb. left. exact F. }
+        intros. eapply marginal_not_bound. { exact I. } apply BoundIn.TFoB. exact B.
+  - econstructor; try solve [apply Map.union_set]; try solve [apply Map.add_set]; try eassumption.
+    + intros k [[] F] I. eapply N. 2: { exact I. } apply U in F as [F | F]. { exists tt. exact F. }
+      edestruct marginal_not_bound as []. { exists tt. exact F. } apply BoundIn.TCaP. apply Bp. exact I.
+    + eapply eq; try reflexivity; try eapply IHL1. 2: { apply Map.union_set. } 3: {
+        eapply Map.union_det; try apply Map.eq_refl. { exact Ab. } apply Map.union_set. } 2: { split.
+        * intro F. apply Map.union_set. apply Map.union_set in F as [F | F]. {
+            apply Cb' in F as [F | F]; [left | right]. { exact F. }
+            apply Map.union_set. apply Cb in F as [F | F]; [left | right]. 2: { exact F. } apply U. left. exact F. }
+          right. apply Map.union_set. left. apply U. right. exact F.
+        * intro F. apply Map.union_set. apply Map.union_set in F as [F | F]. { left. apply Cb'. left. exact F. }
+          apply Map.union_set in F as [F | F]. 2: { left. apply Cb'. right. apply Cb. right. exact F. }
+          apply U in F as [F | F]; [left | right]. 2: { exact F. } apply Cb'. right. apply Cb. left. exact F. }
+        intros. eapply marginal_not_bound. { exact I. } apply BoundIn.TCaB. exact B.
+    + eapply IHL2. 2: { intros k []. split.
+      * intro F. apply Map.union_set in F as [F | F]. 2: { left. apply Co. right. exact F. }
+        apply U in F as [F | F]. 2: { right. exact F. } left. apply Co. left. exact F.
+      * intros FF. apply Map.union_set. destruct FF as [F | F]. 2: { left. apply U. right. exact F. }
+        apply Co in F as [F | F]. 2: { right. exact F. } left. apply U. left. exact F. }
+      intros x I B. eapply marginal_not_bound. { exact I. } apply BoundIn.TCaO. exact B.
+Qed.
+
+Lemma unshadow_acc_cas acc cant_bind pattern body_if_match other_cases
+  : unshadow_acc acc cant_bind (Term.Cas pattern body_if_match other_cases) =
+    match unshadow_acc acc cant_bind other_cases with None => None | Some (cant_bind, other_cases') =>
+      match Rename.pattern (NewNames.generate cant_bind $ BoundIn.pattern pattern) pattern with
+      | None => None
+      | Some pattern' =>
+          match unshadow_acc
+            (Map.bulk_overwrite (NewNames.generate cant_bind $ BoundIn.pattern pattern) acc)
+            (Map.set_union (Map.range $ NewNames.generate cant_bind $ BoundIn.pattern pattern) cant_bind)
+            body_if_match
+          with None => None | Some (cant_bind, body_if_match') =>
+            Some (cant_bind, Term.Cas pattern' body_if_match' other_cases')
+          end
+      end
+    end.
+Proof. reflexivity. Qed.
+
+Lemma on_the_tin_acc {acc cant_bind} (prev : forall x y, Map.Find acc x y -> Map.In cant_bind y)
+  {t cant_bind' t'} (E : unshadow_acc acc cant_bind t = Some (cant_bind', t'))
+  {context} (no_free_vars : forall x (U : UsedIn.Term t' x), Map.In context x)
+  : UnshadowedIn cant_bind context t'.
+Proof.
+  generalize dependent context. generalize dependent t'. generalize dependent cant_bind'.
+  generalize dependent cant_bind. generalize dependent acc. induction t; intros.
+  - cbn in E. invert E. constructor.
+  - cbn in E. destruct Map.find eqn:F in E; invert E. apply Map.find_iff in F. constructor. apply no_free_vars. constructor.
+  - cbn in E. destruct unshadow_acc as [[cant_bind1' t1'] |] eqn:E1 in E. 2: { discriminate E. }
+    destruct unshadow_acc as [[cant_bind2' t2'] |] eqn:E2 in E; invert E. specialize (IHt1 _ _ prev _ _ E1).
+    assert (Eb1 := bindings E1 prev). eassert (prev' : _); [| specialize (IHt2 _ _ prev' _ _ E2)]. {
+      intros. apply Eb1. right. eapply prev. exact H. } assert (Eb2 := bindings E2 prev').
+    econstructor; try solve [apply BoundIn.term_iff]; try solve [apply Map.union_set].
+    + eapply cant_bind_union. 3: { apply Map.union_set. } { eapply IHt1. intros. apply no_free_vars. apply UsedIn.ApF. exact U. }
+      intros x B2 B1. apply BoundIn.term_iff in B2. eapply disj_bound; try eapply IHt2; try exact E2; try eassumption.
+      * intros z U. eapply no_free_vars. apply UsedIn.ApA. exact U.
+      * eapply Eb1. left. exact B1.
+    + eapply eq; try reflexivity; try eapply IHt2; try apply Map.eq_refl. { intros z U. eapply no_free_vars. apply UsedIn.ApA. exact U. }
+      intros x []. rewrite (Map.reflect_find Eb1). assert (US := Map.union_set). cbn in US. rewrite US.
+      split. { intros [B | [[] F]]; [right | left]. { apply BoundIn.term_iff in B as [[] B]. exact B. } exact F. }
+      intros [F | B]; [right | left]. { exists tt. exact F. } apply BoundIn.term_iff. exists tt. exact B.
+  - cbn in E. destruct unshadow_acc as [[cant_bind1' t1'] |] eqn:E1 in E. 2: { discriminate E. }
+    destruct unshadow_acc as [[cant_bind2' t2'] |] eqn:E2 in E; invert E. specialize (IHt1 _ _ prev _ _ E1).
+    assert (Eb1 := bindings E1 prev). eassert (prev' : _); [| specialize (IHt2 _ _ prev' _ _ E2)]. { intros x y F.
+      apply Map.in_overriding_add. apply Map.overwrite_if_present_overwrite in F as [[-> ->] | [N F]]; [left | right]. { reflexivity. }
+      apply Eb1. right. eapply prev. exact F. }
+    econstructor; try solve [apply BoundIn.term_iff]; try solve [apply Map.union_set]; try solve [apply Map.add_set].
+    + intro I. eapply NewNames.not_in_new_name. apply Eb1. right. exact I.
+    + eapply cant_bind_union. 3: { apply Map.union_set. } { eapply IHt1. intros. apply no_free_vars. apply UsedIn.FoT. exact U. }
+      intros x B2 B1. apply BoundIn.term_iff in B2. eapply disj_bound; [apply IHt2 | | exact B2]. { apply UsedIn.term_iff. }
+      apply Map.in_overriding_add. destruct (String.eqb_spec x $ NewNames.new_name cant_bind1' variable). { left. exact e. }
+      right. apply Eb1. left. exact B1.
+    + eapply cant_bind_union; [eapply context_superset; [apply IHt2 |] | |]. 4: {
+        intros k []. split.
+        -- intro F. apply Map.add_set in F as [[-> _] | F]. { left. apply Map.add_set. left. split; reflexivity. }
+           apply Map.union_set in F as [F | F]. 2: { right. exact F. }
+           left. apply Map.add_set. right. edestruct Eb1 as [_ [[] F']]. 2: { exact F'. } right. exists tt. exact F.
+        -- intro FF. apply Map.add_set. destruct FF as [F | F]. 2: { right. apply Map.union_set. right. exact F. }
+           apply Map.add_set in F as [[-> _] | F]. { left. split; reflexivity. }
+           right. apply Map.union_set. edestruct Eb1 as [[B | [[] F']] _]. { exists tt. exact F. } {
+             right. apply BoundIn.term_iff in B as [[] B]. exact B. } left. exact F'. }
+      * intros x U. eapply (Map.in_overriding_add _ _ tt).
+        destruct (String.eqb_spec x $ NewNames.new_name cant_bind1' variable); [left | right]. { exact e. }
+        apply no_free_vars. apply UsedIn.FoB. { exact n. } exact U.
+      * intros k [] F. apply Map.add_set. apply Map.add_set in F. exact F.
+      * intros x B1 B2. apply BoundIn.term_iff in B1. eapply disj_bound; [apply IHt2 | | exact B2]. { apply UsedIn.term_iff. }
+        apply Map.in_overriding_add. destruct (String.eqb_spec x $ NewNames.new_name cant_bind1' variable). { left. exact e. }
+        right. apply Eb1. left. exact B1.
+  - rewrite unshadow_acc_cas in E. destruct unshadow_acc as [[cant_bind2' t2'] |] eqn:E2 in E. 2: { discriminate E. }
+    destruct (Rename.pattern_spec (NewNames.one_to_one_generate cant_bind2' $ BoundIn.pattern pattern) pattern). 2: { discriminate E. }
+    destruct unshadow_acc as [[cant_bind1' t1'] |] eqn:E1 in E; invert E. specialize (IHt2 _ _ prev _ _ E2).
+    assert (Eb2 := bindings E2 prev). eassert (prev' : _); [| specialize (IHt1 _ _ prev' _ _ E1)]. {
+      intros k v F. apply Map.in_overriding_union.
+      apply Map.bulk_overwrite_bulk_overwrite in F as [F | [N F]]; [left | right]. { apply Map.in_range. eexists. exact F. }
+      eapply bindings. { exact E2. } { exact prev. } right. eapply prev. exact F. }
+    econstructor; try solve [apply Map.union_set]; try solve [apply BoundIn.term_iff]; try solve [apply BoundIn.pattern_iff].
+    + intros z I B. apply BoundIn.pattern_iff in B. eapply (Rename.bound_in_pattern Y) in B as [b [B F]].
+      eapply NewNames.not_in_generate. { apply Eb2. right. exact I. } exists b. exact F.
+    + eapply cant_bind_union; [eapply context_superset; [apply IHt1 |] | |]. 4: {
+        intros k []. split.
+        -- intro F. apply Map.union_set in F as [F | F]. { left. apply Map.union_set. left. apply Map.find_range.
+             assert (B : BoundIn.Pattern x k). { apply BoundIn.pattern_iff. exists tt. exact F. }
+             apply (Rename.bound_in_pattern Y) in B as [b [B F']]. exists b. exact F'. }
+           apply Map.union_set in F as [F | F]. 2: { right. exact F. }
+           left. apply Map.union_set. right. edestruct Eb2 as [_ [[] F']]. 2: { exact F'. } right. exists tt. exact F.
+        -- intro FF. apply Map.union_set. destruct FF as [F | F]. 2: { right. apply Map.union_set. right. exact F. }
+           apply Map.union_set in F as [F | F].
+           ++ apply Map.find_range in F as [j F]. left. edestruct BoundIn.pattern_iff as [_ [[] F']]. 2: { exact F'. }
+              eapply (Rename.bound_in_pattern Y). eexists. split. 2: { exact F. }
+              apply BoundIn.pattern_iff. eapply NewNames.in_generate. exists k. exact F.
+           ++ right. apply Map.union_set. edestruct Eb2 as [[B | [[] F']] _]. { exists tt. exact F. } 2: { left. exact F'. }
+              right. apply BoundIn.term_iff in B as [[] B]. exact B. }
+      * intros z U. eapply Map.in_overriding_union.
+        destruct (BoundIn.pattern_spec x z); [left | right]. { apply BoundIn.pattern_iff. exact Y0. }
+        apply no_free_vars. apply UsedIn.CaB. { exact N. } exact U.
+      * intros k [] F. apply Map.union_set. apply Map.union_set in F. exact F.
+      * intros z B2 B1. apply BoundIn.term_iff in B2. eapply disj_bound; [apply IHt1 | | exact B1]. { apply UsedIn.term_iff. }
+        eapply Map.in_overriding_union. destruct (BoundIn.pattern_spec x z); [left | right]. 2: { apply Eb2. left. exact B2. }
+        apply Map.in_range. apply (Rename.bound_in_pattern Y) in Y0 as [b [B F]]. eexists. exact F.
+    + eapply cant_bind_union. 3: { apply Map.union_set. } { eapply IHt2. intros. apply no_free_vars. apply UsedIn.CaO. exact U. }
+      intros z B1 B2. apply BoundIn.term_iff in B1. eapply disj_bound; [apply IHt1 | | exact B1]. { apply UsedIn.term_iff. }
+      eapply Map.in_overriding_union. destruct (BoundIn.pattern_spec x z); [left | right]. 2: { apply Eb2. left. exact B2. }
+      apply Map.in_range. apply (Rename.bound_in_pattern Y) in Y0 as [b [B F]]. eexists. exact F.
+Qed.
+
+Lemma on_the_tin_reserve {cant_bind t t'} (E : unshadow_reserve cant_bind t = Some t')
+  {context} (no_free_vars : forall x (U : UsedIn.Term t' x), Map.In context x)
+  : UnshadowedIn (Map.set_union cant_bind $ Map.range $ NewNames.generate cant_bind $ UsedIn.term t) context t'.
+Proof.
+  unfold unshadow_reserve in E. destruct unshadow_acc as [[] |] eqn:U in E; invert E.
+  eapply on_the_tin_acc. 2: { exact U. } 2: { exact no_free_vars. }
+  intros x y F. apply Map.in_overriding_union. right. apply Map.in_range. exists x. exact F.
+Qed.
+
+Lemma on_the_tin {t t'} (E : unshadow t = Some t')
+  {context} (no_free_vars : forall x (U : UsedIn.Term t' x), Map.In context x)
+  : UnshadowedIn (Map.range $ NewNames.generate Map.empty $ UsedIn.term t) context t'.
+Proof.
+  eapply eq. { eapply on_the_tin_reserve. { exact E. } exact no_free_vars. } 2: { apply Map.eq_refl. } 2: { reflexivity. }
+  intros x []. split. { intro F. apply Map.union_set in F as [F | F]. { invert F. } exact F. }
+  intro F. apply Map.union_set. right. exact F.
+Qed.
+
+
+
+Print UnshadowedIn.
+Fixpoint unshadowed_in (cant_bind context : Map.set) t :=
   match t with
-  | Term.Ctr _ =>
-      Some (Map.empty, Map.empty)
-  | Term.Var name _ =>
-      Some (Map.empty, Map.singleton name tt)
+  | Term.Ctr _ => true
+  | Term.Var name => Map.in_ context name
   | Term.App function argument =>
-      match unshadowed_acc function with None => None | Some (bound_in_function, used_in_function) =>
-      match unshadowed_acc argument with None => None | Some (bound_in_argument, used_in_argument) =>
+      match unshadowed_acc cant_bind context function with None => None | Some (bound_in_function, used_in_function) =>
+      match unshadowed_acc cant_bind context argument with None => None | Some (bound_in_argument, used_in_argument) =>
       if andb
         (Map.disjoint bound_in_function used_in_argument)
         (Map.disjoint bound_in_argument used_in_function)
@@ -550,8 +1715,41 @@ Fixpoint unshadowed_acc t :=
         Map.set_union used_in_argument used_in_function)
       else None end end
   | Term.For variable type body =>
-      match unshadowed_acc type with None => None | Some (bound_in_type, used_in_type) =>
-      match unshadowed_acc body with None => None | Some (bound_in_body, used_in_body) =>
+      if Map.in_ cant_bind variable then None else
+      match unshadowed_acc cant_bind context type with None => None | Some (bound_in_type, used_in_type) =>
+      match unshadowed_acc cant_bind (Map.set_add variable context) body with None => None | Some (bound_in_body, used_in_body) =>
+      if
+        andb (Map.disjoint bound_in_type used_in_body) $
+        andb (Map.disjoint bound_in_body used_in_type) $
+        andb (negb $ Map.in_ bound_in_type variable) $ negb $ Map.in_ bound_in_body variable
+      then Some (
+        Map.set_add variable $ Map.set_union bound_in_type bound_in_body,
+        Map.set_union used_in_type $ Map.remove variable used_in_body)
+      else None end end
+  end.
+
+
+
+Fixpoint unshadowed_acc {T} (cant_bind context : Map.set) t :=
+  match t with
+  | Term.Ctr _ =>
+      Some (Map.empty, Map.empty)
+  | Term.Var name _ =>
+      Some (Map.empty, Map.singleton name tt)
+  | Term.App function argument =>
+      match unshadowed_acc cant_bind context function with None => None | Some (bound_in_function, used_in_function) =>
+      match unshadowed_acc cant_bind context argument with None => None | Some (bound_in_argument, used_in_argument) =>
+      if andb
+        (Map.disjoint bound_in_function used_in_argument)
+        (Map.disjoint bound_in_argument used_in_function)
+      then Some (
+        Map.set_union bound_in_function bound_in_argument,
+        Map.set_union used_in_argument used_in_function)
+      else None end end
+  | Term.For variable type body =>
+      if Map.in_ cant_bind variable then None else
+      match unshadowed_acc cant_bind context type with None => None | Some (bound_in_type, used_in_type) =>
+      match unshadowed_acc cant_bind (Map.set_add variable context) body with None => None | Some (bound_in_body, used_in_body) =>
       if
         andb (Map.disjoint bound_in_type used_in_body) $
         andb (Map.disjoint bound_in_body used_in_type) $
@@ -561,24 +1759,29 @@ Fixpoint unshadowed_acc t :=
         Map.set_union used_in_type $ Map.remove variable used_in_body)
       else None end end
   | Term.Cas pattern body_if_match other_cases =>
-      match unshadowed_acc body_if_match with None => None | Some (bound_in_body_if_match, used_in_body_if_match) =>
-      match unshadowed_acc other_cases with None => None | Some (bound_in_other_cases, used_in_other_cases) =>
       let bound_in_pattern := BoundIn.pattern pattern in
-      if
-        andb (Map.disjoint bound_in_body_if_match used_in_other_cases) $
-        andb (Map.disjoint bound_in_other_cases used_in_body_if_match) $
-        andb (Map.disjoint bound_in_pattern bound_in_body_if_match) $
-        Map.disjoint bound_in_pattern bound_in_other_cases
-      then Some (
-        Map.set_union bound_in_pattern $ Map.set_union bound_in_body_if_match bound_in_other_cases,
-        Map.set_union used_in_other_cases $ Map.minus used_in_body_if_match bound_in_pattern)
-      else None end end
+      if Map.disjoint cant_bind bound_in_pattern then
+        match unshadowed_acc cant_bind body_if_match with None => None | Some (bound_in_body_if_match, used_in_body_if_match) =>
+        match unshadowed_acc cant_bind other_cases with None => None | Some (bound_in_other_cases, used_in_other_cases) =>
+        if
+          andb (Map.disjoint bound_in_body_if_match used_in_other_cases) $
+          andb (Map.disjoint bound_in_other_cases used_in_body_if_match) $
+          andb (Map.disjoint bound_in_pattern bound_in_body_if_match) $
+          Map.disjoint bound_in_pattern bound_in_other_cases
+        then Some (
+          Map.set_union bound_in_pattern $ Map.set_union bound_in_body_if_match bound_in_other_cases,
+          Map.set_union used_in_other_cases $ Map.minus used_in_body_if_match bound_in_pattern)
+        else None end end
+      else None
   end.
 
-Definition unshadowed t := match unshadowed_acc t with None => false | Some _ => true end.
-Arguments unshadowed t/.
+Definition unshadowed_in context t :=
+  match unshadowed_acc context t with None => false | Some (bound, used) =>
+    Map.subset (fun _ _ => true) used context
+  end.
 
-Lemma unshadowed_acc_bound_used {t bound used} (E : unshadowed_acc t = Some (bound, used))
+Lemma unshadowed_acc_bound_used {T} {cant_bind : Map.to T}
+  {t bound used} (E : unshadowed_acc cant_bind t = Some (bound, used))
   : Map.Reflect (BoundIn.Term t) bound /\ Map.Reflect (UsedIn.Term t) used.
 Proof.
   generalize dependent used. generalize dependent bound. induction t; intros; cbn in *.
@@ -609,7 +1812,8 @@ Proof.
       * intro B. apply Map.in_overriding_union. invert B; [right | left].
         -- apply Uf. exact used_in_function0.
         -- apply Ua. exact used_in_argument0.
-  - destruct unshadowed_acc as [[bound_in_type used_in_type] |] eqn:Et in E. 2: { discriminate E. }
+  - destruct Map.find in E. { discriminate E. }
+    destruct unshadowed_acc as [[bound_in_type used_in_type] |] eqn:Et in E. 2: { discriminate E. }
     destruct unshadowed_acc as [[bound_in_body used_in_body] |] eqn:Eb in E. 2: { discriminate E. }
     assert (D := @Map.disjoint_spec unit unit). cbn in D.
     destruct (D bound_in_type used_in_body). 2: { discriminate E. }
@@ -632,7 +1836,8 @@ Proof.
       * intro U. apply Map.in_overriding_union. invert U; [left | right]. { apply Ut. exact used_in_type0. }
         eapply Map.in_remove_if_present. { apply Map.remove_if_present_remove. }
         split. { exact not_shadowed. } apply Ub. exact used_in_body0.
-  - destruct unshadowed_acc as [[bound_in_body_if_match used_in_body_if_match] |] eqn:Eb in E. 2: { discriminate E. }
+  - destruct Map.for_all in E. 2: { discriminate E. }
+    destruct unshadowed_acc as [[bound_in_body_if_match used_in_body_if_match] |] eqn:Eb in E. 2: { discriminate E. }
     destruct unshadowed_acc as [[bound_in_other_cases used_in_other_cases] |] eqn:Eo in E. 2: { discriminate E. }
     assert (D := @Map.disjoint_spec unit unit). cbn in D.
     destruct (D bound_in_body_if_match used_in_other_cases). 2: { discriminate E. }
@@ -656,14 +1861,41 @@ Proof.
         intro B. apply not_shadowed. apply BoundIn.pattern_iff. exact B.
 Qed.
 
+Lemma acc_spec cant_bind context t
+  : Reflect.Option (fun _ => UnshadowedIn cant_bind context t) (unshadowed_acc cant_bind t).
+Proof.
+  generalize dependent context. generalize dependent cant_bind. induction t; intros; cbn in *.
+  - constructor. constructor.
+  - constructor. constructor.
+Qed.
+
+Lemma unshadowed_in_spec context t
+  : Reflect.Bool (UnshadowedIn context t) (unshadowed_in context t).
+Proof.
+  generalize dependent context. induction t; intros; cbn in *.
+  - rewrite Map.for_all_empty. constructor. constructor.
+  - rewrite Map.for_all_singleton. cbn. destruct (Map.find_spec context name); constructor. { constructor. eexists. exact Y. }
+    intro U. invert U. destruct no_free_variables as [y F]. apply N in F as [].
+  - unfold unshadowed_in in *. cbn. specialize (IHt1 context). destruct (unshadowed_acc context t1) as [[bound1 used1] |] eqn:E1. 2: {
+      constructor. intro C. invert C. invert IHt1. apply N; clear N. eapply subset. { exact Uf. } { Search UnshadowedIn UsedIn.Term.
+      invert IHt1. rewrite E1 in H0.
+
+
+
+      apply N in Uf as []. }
+    destruct (unshadowed_acc t2) as [[bound2 used2] |] eqn:E2. 2: {
+      constructor. intro C. invert C. specialize (IHt2 context_argument). invert IHt2. apply N in Ua as []. }
+    asdf.
+Qed.
+
 Lemma unshadowed_spec t
-  : Reflect.Bool (Unshadowed t) (unshadowed t).
+  : Reflect.Bool (UnshadowedIn (UsedIn.term t) t) (unshadowed t).
 Proof.
   induction t; cbn in *.
   - constructor. constructor.
-  - constructor. constructor.
+  - constructor. constructor. apply Map.in_singleton. reflexivity.
   - destruct unshadowed_acc as [[bound_in_function used_in_function] |] eqn:Ef; invert IHt1. 2: {
-      constructor. intro U. apply N. invert U. exact Uf. }
+      constructor. intro U. apply N; clear N. invert U. exact Uf. }
     destruct unshadowed_acc as [[bound_in_argument used_in_argument] |] eqn:Ea at 1; rewrite Ea in IHt2; invert IHt2. 2: {
       constructor. intro U. apply N. invert U. exact Ua. }
     destruct (unshadowed_acc_bound_used Ef) as [Bf Uf]. destruct (unshadowed_acc_bound_used Ea) as [Ba Ua].
@@ -710,6 +1942,7 @@ Qed.
 Lemma unshadowed_iff t
   : Unshadowed t <-> unshadowed t = true.
 Proof. exact (Reflect.bool_iff (unshadowed_spec _)). Qed.
+*)
 
 
 
